o Working on diff_abs_bot.

continuity/continuity_defs.v
@@ -35,9 +35,8 @@ Require Export alphaeq2.
 Require Export substitution2.
 Require Export terms4.
 Require Export computation10.
+Require Export computation11.
 Require Export nat_defs.
-
-
 
 
 Definition uexc {o} (a : get_patom_set o) :=
@@ -182,46 +181,6 @@ Proof.
   - apply alphaeqbt_nilv2; auto.
 Qed.
 
-Definition br_list {T} R (l1 l2 : list T) :=
-  length l1 = length l2
-  # (forall a1 a2,
-       LIn (a1,a2) (combine l1 l2)
-       -> R a1 a2).
-
-Definition br_bterms {o} R (bs1 bs2 : list (@BTerm o)) := br_list R bs1 bs2.
-
-Lemma br_bterms_nil {o} :
-  forall (R : @BTerm o -> @BTerm o -> Type),
-    br_bterms R [] [].
-Proof.
-  introv.
-  unfold br_bterms, br_list; simpl; sp.
-Qed.
-Hint Resolve br_bterms_nil : slow.
-
-Lemma br_bterms_cons {o} :
-  forall R (b1 b2 : @BTerm o) bs1 bs2,
-    R b1 b2
-    -> br_bterms R bs1 bs2
-    -> br_bterms R (b1 :: bs1) (b2 :: bs2).
-Proof.
-  introv h1 h2.
-  allunfold @br_bterms.
-  allunfold @br_list; simpl; tcsp.
-  dands; tcsp.
-  introv i; dorn i; cpx; tcsp.
-Qed.
-Hint Resolve br_bterms_cons : slow.
-
-Lemma alpha_eq_bterms_implies_same_length {o} :
-  forall (bs1 bs2 : list (@BTerm o)),
-    alpha_eq_bterms bs1 bs2 -> length bs1 = length bs2.
-Proof.
-  introv aeq.
-  unfold alpha_eq_bterms, br_bterms, br_list in aeq; sp.
-Qed.
-Hint Resolve alpha_eq_bterms_implies_same_length : slow.
-
 Lemma alpha_eq_force_int_bound {o} :
   forall b v1 v2 (t1 t2 e1 e2 : @NTerm o),
     !LIn v1 (free_vars e1)
@@ -269,1290 +228,6 @@ Proof.
       allrw disjoint_singleton_r; auto.
 Qed.
 
-Lemma alpha_bterm_change_aux {o} :
-  forall (bt : @BTerm o) lv nt lvn,
-  alpha_eq_bterm bt (bterm lv nt)
-  -> disjoint (all_vars nt) lvn
-  -> no_repeats lvn
-  -> length lv = length lvn
-  -> alpha_eq_bterm bt (bterm lvn (lsubst_aux nt (var_ren lv lvn))).
-Proof.
-  introv aeq disj norep len.
-  pose proof (alpha_bterm_change
-                bt lv nt lvn
-                aeq disj norep len) as h.
-  unfold lsubst in h; simpl h; boolvar; auto.
-  provefalse; destruct n.
-  rw @range_var_ren; auto.
-  rw flat_map_map.
-  unfold compose.
-  rw disjoint_flat_map_r; introv i; simpl.
-  rw disjoint_singleton_r; intro k.
-  apply disjoint_sym in disj; apply disj in i.
-  rw in_app_iff in i; rw not_over_or in i; sp.
-Qed.
-
-Lemma implies_eqvars_flat_map_diff :
-  forall (A : tuniv) (f g : A -> list NVar) (l k : list A),
-    length l = length k
-    -> (forall x y : A, LIn (x,y) (combine l k) -> eqvars (f x) (g y))
-    -> eqvars (flat_map f l) (flat_map g k).
-Proof.
-  induction l; destruct k; introv len imp; allsimpl; cpx.
-  apply eqvars_app; auto.
-Qed.
-
-Lemma fresh_var_lt :
-  forall vs v,
-    (forall x, LIn (nvar x) vs -> v < x)
-    -> fresh_var_aux v vs = v.
-Proof.
-  induction vs; introv i; allsimpl; tcsp.
-  destruct a.
-  boolvar; auto; subst.
-  pose proof (i n) as h; autodimp h hyp; sp.
-Qed.
-
-Lemma le_var_implies_eq :
-  forall a b, le_var a b -> le_var b a -> a = b.
-Proof.
-  introv k1 k2.
-  destruct a, b.
-  allunfold le_var.
-  f_equal; omega.
-Qed.
-
-Inductive sublist {T} : list T -> list T -> Type :=
-| sublist_nil : sublist [] []
-| sublist_cons :
-    forall t l1 l2,
-      sublist l1 l2
-      -> sublist (t :: l1) (t :: l2)
-| sublist_tl :
-    forall t l1 l2,
-      sublist l1 l2
-      -> sublist l1 (t :: l2).
-Hint Constructors sublist.
-
-Lemma sublist_refl :
-  forall T (l : list T),
-    sublist l l.
-Proof.
-  induction l; auto.
-Qed.
-
-Lemma list_ind_sublist :
-  forall (A : Type) (P : list A -> Type),
-    P []
-    -> (forall (l : list A),
-          (forall (k : list A),
-             length k < length l
-             -> sublist k l
-             -> P k)
-          -> P l)
-    -> forall l : list A, P l.
-Proof.
-  introv nc sc; introv.
-  assert ({n | length l = n}) as e by (exists (length l); auto); sp.
-  revert l e.
-  induction n as [n Hind] using comp_ind_type; introv len; cpx.
-  destruct n; cpx.
-  destruct l; allsimpl; cpx.
-  apply (sc (a :: l)); allsimpl; tcsp.
-  introv i s.
-  apply (Hind (length k)); auto.
-Qed.
-
-Tactic Notation "sublist_ind" ident(h) ident(c) :=
-  induction h using list_ind_sublist;
-  [ Case_aux c "nil"
-  | Case_aux c "cons"
-  ].
-
-Tactic Notation "sublist_ind" ident(h) "as" simple_intropattern(I) ident(c) :=
-  induction h as I using list_ind_sublist;
-  [ Case_aux c "nil"
-  | Case_aux c "cons"
-  ].
-
-Lemma issorted_eqvars :
-  forall l1 l2 x,
-    issorted (x :: l1)
-    -> issorted l2
-    -> eqvars (x :: l1) l2
-    -> {l1h : list NVar
-        & {l1t : list NVar
-        & {l2h : list NVar
-        & {l2t : list NVar
-        & l1 = l1h ++ l1t
-        # l2 = l2h ++ l2t
-        # (forall t, LIn t l1h -> t = x)
-        # (forall t, LIn t l2h -> t = x)
-        # !LIn x l1t
-        # !LIn x l2t
-        # eqvars l1t l2t}}}}.
-Proof.
-  sublist_ind l1 as [|l1 ind] Case; destruct l2; introv iss1 iss2 eqv; allsimpl.
-
-  - apply eqvars_sym in eqv.
-    apply eqvars_nil in eqv; cpx.
-
-  - exists ([] : list NVar) ([] : list NVar) (n :: l2) ([] : list NVar); simpl.
-    allrw app_nil_r; dands; tcsp.
-    rw eqvars_prop in eqv.
-    introv i; dorn i; subst; auto.
-
-    + pose proof (eqv t) as h; destruct h as [h1 h]; clear h1.
-      simpl in h; sp.
-
-    + pose proof (eqv t) as h; destruct h as [h1 h]; clear h1.
-      simpl in h; sp.
-
-  - apply eqvars_sym in eqv.
-    apply eqvars_nil in eqv; cpx.
-
-  - inversion iss1 as [|? ? h1 h2]; subst.
-    assert (x = n) as e.
-
-    + rw eqvars_prop in eqv.
-
-      pose proof (eqv x) as k1.
-      destruct k1 as [k1 k]; clear k.
-      simpl in k1; autodimp k1 hyp.
-
-      pose proof (eqv n) as k2.
-      destruct k2 as [k k2]; clear k.
-      simpl in k2; autodimp k2 hyp.
-
-      dorn k2; auto.
-      pose proof (h1 n) as h; simpl in h; autodimp h hyp.
-      dorn k1; auto.
-      inversion iss2 as [|? ? p1 p2]; subst.
-      apply p1 in k1.
-      apply le_var_implies_eq; auto.
-
-    + subst.
-      pose proof (eqvars_remove_nvar (n :: l1) (n :: l2) n eqv) as h.
-      allrw (remove_nvar_cons n n); boolvar.
-      inversion iss2 as [|? ? k1 k2]; subst.
-Abort.
-
-Definition remove_repeated_vars := remove_repeats deq_nvar.
-Hint Unfold remove_repeated_vars.
-
-Lemma fresh_var_aux_eq_S :
-  forall vs n,
-    issorted vs
-    -> LIn (nvar n) vs
-    -> fresh_var_aux (S n) vs = fresh_var_aux n vs.
-Proof.
-  induction vs; introv iss i; allsimpl; tcsp.
-  destruct a.
-  inversion iss as [|? ? imp iss1]; subst; clear iss.
-  boolvar; tcsp; try omega.
-  - provefalse.
-    dorn i; ginv; try omega.
-    discover.
-    allunfold le_var; allsimpl; omega.
-  - subst.
-    provefalse.
-    dorn i; ginv.
-    + inversion i; omega.
-    + discover.
-      allunfold le_var; omega.
-  - dorn i; ginv; auto; omega.
-Qed.
-
-Lemma eq_fresh_var_aux_remove_repeated :
-  forall vs n,
-    issorted vs
-    -> fresh_var_aux n vs = fresh_var_aux n (remove_repeated_vars vs).
-Proof.
-  induction vs; introv iss; simpl; auto.
-  destruct a.
-  inversion iss as [|? ? imp iss1]; subst; clear iss.
-  allunfold remove_repeated_vars; simpl.
-  boolvar; auto; simpl; boolvar; tcsp; subst.
-
-  - rw fresh_var_lt; auto.
-    introv i.
-    allrw in_remove_repeats.
-    discover.
-    allunfold le_var; omega.
-
-  - rw <- IHvs; auto.
-    apply fresh_var_aux_eq_S; auto.
-Qed.
-
-Lemma issorted_remove_repeated_vars :
-  forall l, issorted l -> issorted (remove_repeated_vars l).
-Proof.
-  induction l; introv iss; allunfold remove_repeated_vars; allsimpl; auto.
-  inversion iss as [|? ? imp iss1]; subst; clear iss.
-  boolvar; auto.
-  constructor; auto.
-  introv i.
-  allrw in_remove_repeats.
-  discover; auto.
-Qed.
-
-Lemma eqvars_remove_repeated_vars :
-  forall l1 l2,
-    eqvars l1 l2
-    -> eqvars (remove_repeated_vars l1) l2.
-Proof.
-  introv eqv.
-  allrw eqvars_prop.
-  introv.
-  unfold remove_repeated_vars.
-  rw in_remove_repeats; auto.
-Qed.
-
-Lemma no_repeats_remove_repeated_vars :
-  forall vs, no_repeats (remove_repeated_vars vs).
-Proof.
-  introv; apply no_repeats_remove_repeats.
-Qed.
-
-Lemma if_eqvars_cons :
-  forall v vs1 vs2,
-    !LIn v vs1
-    -> !LIn v vs2
-    -> eqvars (v :: vs1) (v :: vs2)
-    -> eqvars vs1 vs2.
-Proof.
-  introv ni1 ni2 eqv.
-  allrw eqvars_prop.
-  introv.
-  pose proof (eqv x) as h; destruct h as [h1 h2]; allsimpl.
-  split; introv i.
-  - autodimp h1 hyp; dorn h1; subst; tcsp.
-  - autodimp h2 hyp; dorn h2; subst; tcsp.
-Qed.
-
-Lemma eq_vars_if_issorted_no_repeats_and_eqvars :
-  forall vs1 vs2,
-    issorted vs1
-    -> issorted vs2
-    -> eqvars vs1 vs2
-    -> no_repeats vs1
-    -> no_repeats vs2
-    -> vs1 = vs2.
-Proof.
-  induction vs1; introv iss1 iss2 eqv norep1 norep2; allsimpl; tcsp.
-  - apply eqvars_nil in eqv; subst; auto.
-  - inversion norep1 as [|? ? ni1 nr1]; subst; clear norep1.
-    inversion iss1 as [|? ? imp1 is1]; subst; clear iss1.
-    destruct vs2.
-    + apply eqvars_sym in eqv; apply eqvars_nil in eqv; sp.
-    + inversion norep2 as [|? ? ni2 nr2]; subst; clear norep2.
-      inversion iss2 as [|? ? imp2 is2]; subst; clear iss2.
-
-      dup eqv as i.
-      rw eqvars_prop in i.
-
-      pose proof (i a) as h1; destruct h1 as [h1 h]; clear h.
-      simpl in h1; autodimp h1 hyp.
-
-      pose proof (i n) as h2; destruct h2 as [h h2]; clear h.
-      simpl in h2; autodimp h2 hyp.
-
-      dorn h1; subst;[|dorn h2; subst].
-
-      * clear h2.
-        apply if_eqvars_cons in eqv; auto.
-        f_equal.
-        apply IHvs1; auto.
-
-      * apply if_eqvars_cons in eqv; auto.
-        f_equal.
-        apply IHvs1; auto.
-
-      * discover.
-        assert (a = n) as e.
-        { destruct a, n; allunfold le_var; allsimpl; f_equal; omega. }
-
-        subst.
-        apply if_eqvars_cons in eqv; auto.
-        f_equal.
-        apply IHvs1; auto.
-Qed.
-
-Lemma eq_fresh_var :
-  forall vs1 vs2,
-    eqvars vs1 vs2
-    -> fresh_var vs1 = fresh_var vs2.
-Proof.
-  introv eqv.
-  unfold fresh_var.
-  remember 0 as n; clear Heqn.
-  f_equal.
-  remember (sort vs1) as l1.
-  remember (sort vs2) as l2.
-  pose proof (sort_eqvars vs1) as e1.
-  rw <- Heql1 in e1.
-  pose proof (sort_eqvars vs2) as e2.
-  rw <- Heql2 in e2.
-  pose proof (sort_issorted vs1) as i1.
-  rw <- Heql1 in i1.
-  pose proof (sort_issorted vs2) as i2.
-  rw <- Heql2 in i2.
-  assert (eqvars l1 l2) as ev.
-  eapply eqvars_trans;[|exact e2].
-  eapply eqvars_trans;[|exact eqv].
-  apply eqvars_sym; auto.
-  clear dependent vs1.
-  clear dependent vs2.
-
-  rw (eq_fresh_var_aux_remove_repeated l1); auto.
-  rw (eq_fresh_var_aux_remove_repeated l2); auto.
-  apply issorted_remove_repeated_vars in i1.
-  apply issorted_remove_repeated_vars in i2.
-  apply eqvars_remove_repeated_vars in ev.
-  apply eqvars_sym in ev.
-  apply eqvars_remove_repeated_vars in ev.
-  apply eqvars_sym in ev.
-  pose proof (no_repeats_remove_repeated_vars l1) as nr1.
-  pose proof (no_repeats_remove_repeated_vars l2) as nr2.
-  remember (remove_repeated_vars l1) as vs1.
-  remember (remove_repeated_vars l2) as vs2.
-  clear dependent l1.
-  clear dependent l2.
-
-  apply eq_vars_if_issorted_no_repeats_and_eqvars in ev; auto.
-  rw ev; auto.
-Qed.
-
-
-Lemma fresh_distinct_vars_if_eqvars :
-  forall n vs1 vs2,
-    eqvars vs1 vs2
-    -> fresh_distinct_vars n vs1 = fresh_distinct_vars n vs2.
-Proof.
-  induction n; introv eqv; simpl; auto.
-  rw (eq_fresh_var vs1 vs2); auto.
-  f_equal; auto.
-  apply IHn.
-  apply eqvars_cons_lr; auto.
-Qed.
-
-Lemma br_bterms_cons_iff {o} :
-  forall R (b1 b2 : @BTerm o) bs1 bs2,
-    br_bterms R (b1 :: bs1) (b2 :: bs2)
-    <=> (R b1 b2 # br_bterms R bs1 bs2).
-Proof.
-  introv.
-  allunfold @br_bterms.
-  allunfold @br_list.
-  split; intro k; repnd; dands; allsimpl; cpx.
-  introv i; dorn i; cpx; tcsp.
-Qed.
-
-Lemma matching_bterms_implies_eq_length {o} :
-  forall vars (bs : list (@BTerm o)),
-    matching_bterms vars bs
-    -> length vars = length bs.
-Proof.
-  introv m.
-  unfold matching_bterms in m.
-  rw <- (map_length (fun v : NVar # nat => snd v)).
-  rw <- (map_length num_bvars bs).
-  rw m; auto.
-Qed.
-
-Lemma all_fo_vars_eqvars {o} :
-  forall (t : @SOTerm o),
-    eqvars
-      (all_fo_vars t)
-      (fo_bound_vars t ++ sovars2vars (so_free_vars t)).
-Proof.
-  soterm_ind t as [v ts ind| |op bs ind] Case; simpl; auto.
-
-  - Case "sovar".
-    eapply eqvars_trans;[|apply eqvars_move_around].
-    apply eqvars_cons_lr.
-    rw eqvars_prop; introv; split; intro k; allrw in_app_iff; allrw lin_flat_map; exrepnd.
-    + applydup ind in k1; allrw eqvars_prop.
-      apply k2 in k0; allrw in_app_iff.
-      dorn k0.
-      * left.
-        exists x0; sp.
-      * right.
-        rw sovars2vars_flat_map.
-        rw lin_flat_map.
-        exists x0; sp.
-    + dorn k; exrepnd.
-      * applydup ind in k1.
-        exists x0; dands; auto.
-        rw eqvars_prop in k2.
-        apply k2; rw in_app_iff; tcsp.
-      * rw sovars2vars_flat_map in k.
-        rw lin_flat_map in k; exrepnd.
-        exists x0; dands; auto.
-        applydup ind in k1.
-        rw eqvars_prop in k2.
-        apply k2; rw in_app_iff; tcsp.
-
-  - Case "soterm".
-    induction bs; simpl; auto.
-    autodimp IHbs hyp.
-    { introv i; eapply ind; simpl; eauto. }
-    rw sovars2vars_app.
-    destruct a as [l t].
-    pose proof (ind t l) as h; simpl in h; autodimp h hyp; clear ind.
-    allrw eqvars_prop; introv; simpl.
-    allrw in_app_iff.
-    rw h; clear h.
-    rw IHbs; clear IHbs.
-    allrw in_app_iff.
-    split; intro k; repnd.
-    + dorn k;[dorn k|dorn k]; tcsp.
-      dorn k; tcsp.
-      destruct (in_deq NVar deq_nvar x l); tcsp.
-      right; left.
-      allrw in_sovars2vars; exrepnd.
-      exists n0.
-      rw in_remove_so_vars; dands; auto.
-      intro k.
-      rw in_vars2sovars in k; repnd; subst; sp.
-    + dorn k;[dorn k;[dorn k|]|]; tcsp.
-      dorn k; tcsp.
-      left; right; right.
-      allrw in_sovars2vars; exrepnd.
-      allrw in_remove_so_vars; repnd.
-      exists n; sp.
-Qed.
-
-Lemma eqvars_app_r_implies_subvars :
-  forall vs1 vs2 vs3,
-    eqvars vs1 (vs2 ++ vs3)
-    -> (subvars vs2 vs1 # subvars vs3 vs1).
-Proof.
-  introv e; allrw eqvars_prop; allrw subvars_prop; dands; introv i; apply e;
-  rw in_app_iff; sp.
-Qed.
-
-Lemma compute_step_lib_if_found_entry {o} :
-  forall (lib : library)
-         (oa1 oa2 : opabs)
-         (bs : list BTerm)
-         (vars : list sovar_sig)
-         (rhs : @SOTerm o)
-         (correct : correct_abs oa2 vars rhs),
-    found_entry lib oa1 bs oa2 vars rhs correct
-    -> compute_step_lib lib oa1 bs = csuccess (mk_instance vars bs rhs).
-Proof.
-  introv fe.
-  eapply compute_step_lib_success_change_bs; eauto.
-Qed.
-
-Lemma can_doesnt_reduce_to_exc {o} :
-  forall lib can (l1 l2 : list (@BTerm o)),
-    reduces_to lib (oterm (Can can) l1) (oterm Exc l2)
-    -> False.
-Proof.
-  introv r.
-  unfold reduces_to in r; exrepnd.
-  revert dependent l2.
-  revert dependent l1.
-  induction k; introv r.
-  - rw @reduces_in_atmost_k_steps_0 in r; ginv.
-  - rw @reduces_in_atmost_k_steps_S in r; exrepnd.
-    csunf r1; simpl in r1; ginv.
-    apply IHk in r0; sp.
-Qed.
-
-Definition converges_to_can_or_exc {o} lib (t : @NTerm o) :=
-  {u : NTerm & reduces_to lib t u # is_can_or_exc u}.
-
-Lemma converges_to_value_like_narithop1 {o} :
-  forall (lib : @library o) a bs,
-    converges_to_value_like
-      lib
-      (oterm (NCan (NArithOp a)) bs)
-    -> {t1 : NTerm
-        & {t2 : NTerm
-        & {z1 : Z
-        & {z2 : Z
-        & bs = [nobnd t1, nobnd t2]
-        # reduces_to lib t1 (mk_integer z1)
-        # reduces_to lib t2 (mk_integer z2)
-       }}}}
-       [+]
-       {t : NTerm
-        & {e : NTerm
-        & {l : list BTerm
-        & bs = nobnd t :: l
-        # reduces_to lib t e
-        # isexc e
-       }}}
-       [+]
-       {t1 : NTerm
-        & {t2 : NTerm
-        & {z : Z
-        & {e : NTerm
-        & {l : list BTerm
-        & bs = nobnd t1 :: nobnd t2 :: l
-        # reduces_to lib t1 (mk_integer z)
-        # reduces_to lib t2 e
-        # isexc e
-       }}}}}.
-Proof.
-  introv conv.
-  unfold converges_to_value_like, reduces_to in conv; exrepnd.
-  revert dependent u.
-  revert dependent bs.
-  induction k; introv comp isv.
-
-  - rw @reduces_in_atmost_k_steps_0 in comp; subst.
-    provefalse; unfold isvalue_like in isv; sp.
-
-  - rw @reduces_in_atmost_k_steps_S in comp; exrepnd.
-    destruct bs; ginv.
-    destruct b; ginv.
-    destruct l; ginv.
-    destruct n; ginv.
-    dopid o0 as [can2|ncan2|exc2|abs2] Case; ginv.
-
-    + Case "Can".
-      destruct bs; ginv; try (complete (csunf comp1; allsimpl; dcwf h));[].
-      destruct b.
-      destruct l0; destruct n; try (complete (csunf comp1; allsimpl; dcwf h));[].
-      dopid o0 as [can3|ncan3|exc3|abs3] SCase; ginv.
-
-      * SCase "Can".
-        allsimpl.
-        destruct l; try (complete (csunf comp1; allsimpl; dcwf h));[].
-        destruct l0; try (complete (csunf comp1; allsimpl; dcwf h));[].
-        destruct bs; try (complete (csunf comp1; allsimpl; dcwf h));[].
-        csunf comp1; allsimpl.
-        dcwf h.
-        apply compute_step_arithop_success_can_can in comp1; repnd; GC; exrepnd.
-        allrw @get_param_from_cop_some; allsimpl; subst.
-
-        left.
-
-        exists (@mk_integer o n1) (@mk_integer o n2) n1 n2; dands; tcsp;
-        apply computes_to_value_isvalue_refl;
-        repeat constructor; simpl; sp.
-
-      * SCase "NCan".
-        rw @compute_step_narithop_ncan2 in comp1.
-        dcwf h.
-        remember (compute_step lib (oterm (NCan ncan3) l0)) as c;
-          symmetry in Heqc; destruct c; ginv.
-        apply IHk in comp0; auto; exrepnd; cpx; GC;[].
-        repndors; exrepnd; cpx; GC.
-
-        { left.
-          exists (oterm (Can can2) l) (oterm (NCan ncan3) l0) z1 z2; dands; tcsp.
-          eapply reduces_to_if_split2; eauto. }
-
-        { provefalse.
-          allapply @isexc_implies2; exrepnd; subst.
-          apply can_doesnt_reduce_to_exc in comp2; sp. }
-
-        { right; right.
-          allunfold @ca_wf_def; exrepnd; subst.
-          exists (@mk_integer o i)
-                 (oterm (NCan ncan3) l0)
-                 i e l1;
-            dands; tcsp; eauto with slow.
-          eapply reduces_to_if_split2; eauto. }
-
-      * SCase "Exc".
-        csunf comp1; allsimpl; dcwf h; ginv.
-        allunfold @ca_wf_def; exrepnd; subst.
-        right; right.
-        exists (@mk_integer o i)
-               (oterm Exc l0)
-               i
-               (oterm Exc l0) bs; dands; tcsp; eauto with slow.
-
-      * SCase "Abs".
-        rw @compute_step_narithop_abs2 in comp1.
-        dcwf h;[].
-        remember (compute_step_lib lib abs3 l0) as c.
-        symmetry in Heqc; destruct c; ginv.
-        apply IHk in comp0; auto; exrepnd; cpx; GC.
-        repndors; exrepnd; cpx; GC.
-
-        { left.
-          exists (oterm (Can can2) l) (oterm (Abs abs3) l0) z1 z2; dands; tcsp.
-          eapply reduces_to_if_split2; eauto. }
-
-        { provefalse.
-          allapply @isexc_implies2; exrepnd; subst.
-          apply can_doesnt_reduce_to_exc in comp2; sp. }
-
-        { right; right.
-          allunfold @ca_wf_def; exrepnd; subst.
-          exists (@mk_integer o i)
-                 (oterm (Abs abs3) l0)
-                 i e l1; dands; tcsp; eauto with slow.
-          eapply reduces_to_if_split2; eauto. }
-
-    + Case "NCan".
-      rw @compute_step_narithop_ncan1 in comp1.
-      remember (compute_step lib (oterm (NCan ncan2) l)) as c;
-        symmetry in Heqc; destruct c; ginv.
-      apply IHk in comp0; auto; exrepnd; cpx; GC.
-      dorn comp0;[|dorn comp0]; exrepnd; cpx; GC.
-
-      { left.
-        exists (oterm (NCan ncan2) l) t2 z1 z2; dands; tcsp.
-        eapply reduces_to_if_split2; eauto. }
-
-      { right; left.
-        exists (oterm (NCan ncan2) l) e l0; dands; tcsp.
-        eapply reduces_to_if_split2; eauto. }
-
-      { right; right.
-        exists (oterm (NCan ncan2) l)
-               t2
-               z e l0; dands; tcsp; eauto with slow.
-        eapply reduces_to_if_split2; eauto. }
-
-    + Case "Exc".
-      simpl in comp1.
-      unfold compute_step_catch in comp1; ginv.
-      right; left.
-      exists (oterm Exc l) (oterm Exc l) bs; dands; tcsp; eauto with slow.
-
-    + Case "Abs".
-      rw @compute_step_narithop_abs1 in comp1.
-      remember (compute_step_lib lib abs2 l) as c.
-      symmetry in Heqc; destruct c; ginv.
-      apply IHk in comp0; auto; exrepnd; cpx; GC.
-      dorn comp0;[|dorn comp0]; exrepnd; cpx; GC.
-
-      { left.
-        exists (oterm (Abs abs2) l) t2 z1 z2; dands; tcsp.
-        eapply reduces_to_if_split2; eauto. }
-
-      { right; left.
-        exists (oterm (Abs abs2) l) e l0; dands; tcsp.
-        eapply reduces_to_if_split2; eauto. }
-
-      { right; right.
-        exists (oterm (Abs abs2) l)
-               t2 z e l0; dands; tcsp; eauto with slow.
-        eapply reduces_to_if_split2; eauto. }
-Qed.
-
-Lemma converges_to_can_or_exc_implies_converges_to_value_like {o} :
-  forall lib (t : @NTerm o),
-    converges_to_can_or_exc lib t
-    -> converges_to_value_like lib t.
-Proof.
-  introv c.
-  unfold converges_to_can_or_exc in c.
-  unfold converges_to_value_like.
-  exrepnd; exists u; dands; eauto with slow.
-Qed.
-Hint Resolve converges_to_can_or_exc_implies_converges_to_value_like : slow.
-
-Lemma abs_of_neg :
-  forall z b,
-    (z < 0)%Z
-    -> (- z < Z.of_nat b)%Z
-    -> Z.abs_nat z < b.
-Proof.
-  introv h1 h2.
-  pose proof (Zabs.Zabs_nat_lt (-z) (Z.of_nat b)) as k.
-  autodimp k hyp; try omega.
-  allrw Znat.Zabs2Nat.id.
-  destruct z; allsimpl; try omega.
-Qed.
-
-Lemma abs_of_pos :
-  forall z b,
-    (0 <= z)%Z
-    -> (z < Z.of_nat b)%Z
-    -> Z.abs_nat z < b.
-Proof.
-  introv h1 h2.
-  pose proof (Zabs.Zabs_nat_lt z (Z.of_nat b)) as k.
-  autodimp k hyp; try omega.
-  allrw Znat.Zabs2Nat.id.
-  destruct z; allsimpl; try omega.
-Qed.
-
-Lemma reduces_to_int_subst_less_bound {o} :
-  forall lib b v a can z (bs : list (@BTerm o)),
-    reduces_to
-      lib
-      (subst (less_bound b (mk_var v) (uexc a)) v (oterm (Can can) bs))
-      (mk_integer z)
-    -> can = Nint z # bs = [] # Z.abs_nat z < b.
-Proof.
-  introv r.
-  unfold subst, lsubst in r; allsimpl; boolvar.
-  fold_terms.
-
-  apply reduces_to_split2 in r; dorn r; allsimpl; exrepnd; ginv.
-  csunf r1; allsimpl.
-  unfold on_success in r1.
-  csunf r1; allsimpl.
-  dcwf h; allsimpl.
-  unfold compute_step_comp in r1.
-  destruct bs; allsimpl; ginv.
-  remember (get_param_from_cop can) as g; symmetry in Heqg; destruct g; ginv.
-  destruct p; ginv.
-  allapply @get_param_from_cop_pki; subst.
-
-  apply reduces_to_split2 in r0; dorn r0; allsimpl; exrepnd; ginv.
-  csunf r0; allsimpl.
-  boolvar; allsimpl; ginv.
-
-  - apply reduces_to_split2 in r1; dorn r1; ginv.
-    exrepnd; allsimpl.
-    csunf r1; allsimpl.
-    dcwf h; allsimpl.
-    unfold compute_step_comp in r1; allsimpl; ginv.
-    boolvar; allsimpl.
-
-    + apply reduces_to_if_isvalue_like in r0; eauto with slow.
-      inversion r0; subst; dands; auto.
-      apply abs_of_neg; auto.
-
-    + apply reduces_to_if_isvalue_like in r0; eauto with slow.
-      inversion r0.
-
-  - dcwf h; allsimpl.
-    unfold compute_step_comp in r0; allsimpl; ginv.
-    boolvar; allsimpl.
-
-    + apply reduces_to_if_isvalue_like in r1; eauto with slow.
-      inversion r1; subst; dands; auto.
-      apply abs_of_pos; auto.
-
-    + apply reduces_to_if_isvalue_like in r1; eauto with slow.
-      inversion r1.
-Qed.
-
-Lemma abs_of_neg2 :
-  forall z b,
-    (z < 0)%Z
-    -> Z.abs_nat z < b
-    -> (- z < Z.of_nat b)%Z.
-Proof.
-  introv h1 h2.
-  destruct (Z_lt_le_dec (- z) (Z.of_nat b)) as [h|h]; auto.
-  provefalse.
-  pose proof (Zabs.Zabs_nat_le (Z.of_nat b) (-z)) as k.
-  autodimp k hyp; try omega.
-  allrw Znat.Zabs2Nat.id.
-  destruct z; allsimpl; try omega.
-Qed.
-
-Lemma abs_of_pos2 :
-  forall z b,
-    (0 <= z)%Z
-    -> Z.abs_nat z < b
-    -> (z < Z.of_nat b)%Z.
-Proof.
-  introv h1 h2.
-  destruct (Z_lt_le_dec z (Z.of_nat b)) as [h|h]; auto.
-  provefalse.
-  pose proof (Zabs.Zabs_nat_le (Z.of_nat b) z) as k.
-  autodimp k hyp; try omega.
-  allrw Znat.Zabs2Nat.id.
-  destruct z; allsimpl; try omega.
-Qed.
-
-Definition has_value_like_except {p} lib a (t : @NTerm p) :=
-  {u : NTerm
-   & reduces_to lib t u
-   # isvalue_like u
-   # !isnexc lib a u}.
-
-Lemma has_value_like_except_subst_less_bound {o} :
-  forall lib b v a can (bs : list (@BTerm o)),
-    has_value_like_except
-      lib a
-      (subst (less_bound b (mk_var v) (uexc a)) v (oterm (Can can) bs))
-    -> {z : Z & can = Nint z # bs = [] # Z.abs_nat z < b}.
-Proof.
-  introv r.
-  unfold subst, lsubst in r; allsimpl; boolvar.
-  fold_terms.
-  unfold has_value_like_except in r; exrepnd.
-
-  apply reduces_to_split2 in r1; dorn r1; allsimpl; exrepnd; subst.
-
-  { unfold isvalue_like in r2; exrepnd; repndors; inversion r2. }
-
-  csunf r1; allsimpl.
-  unfold on_success in r1.
-  csunf r1; allsimpl.
-  dcwf h; allsimpl.
-  unfold compute_step_comp in r1.
-  destruct bs; allsimpl; ginv.
-  remember (get_param_from_cop can) as g; symmetry in Heqg; destruct g; ginv.
-  destruct p; ginv.
-  allapply @get_param_from_cop_pki; subst.
-
-  apply reduces_to_split2 in r3; dorn r3; allsimpl; exrepnd; subst.
-
-  { unfold isvalue_like in r2; exrepnd; repndors; inversion r2. }
-
-  csunf r3; allsimpl; boolvar; allsimpl; ginv.
-
-  - apply reduces_to_split2 in r1; dorn r1; allsimpl; exrepnd; subst.
-
-    { unfold isvalue_like in r2; exrepnd; repndors; inversion r2. }
-
-    csunf r1; allsimpl.
-    dcwf h; allsimpl.
-    unfold compute_step_comp in r1; allsimpl; ginv.
-    boolvar; allsimpl.
-
-    + apply reduces_to_if_isvalue_like in r3; eauto with slow; subst.
-      exists z; dands; auto.
-      apply abs_of_neg; auto.
-
-    + apply reduces_to_if_isvalue_like in r3; eauto with slow; subst.
-      destruct r0; simpl; exists (mk_utoken a); simpl; boolvar; dands; tcsp; eauto with slow.
-
-  - dcwf h; allsimpl.
-    unfold compute_step_comp in r3; allsimpl; ginv.
-    boolvar; allsimpl.
-
-    + apply reduces_to_if_isvalue_like in r1; eauto with slow; subst.
-      exists z; dands; auto.
-      apply abs_of_pos; auto.
-
-    + apply reduces_to_if_isvalue_like in r1; eauto with slow; subst.
-      destruct r0; simpl; exists (mk_utoken a); simpl; boolvar; dands; tcsp; eauto with slow.
-Qed.
-
-Lemma hasvalue_like_subst_less_bound {o} :
-  forall lib b v can (bs : list (@BTerm o)),
-    hasvalue_like
-      lib
-      (subst (less_bound b (mk_var v) (mk_vbot v)) v (oterm (Can can) bs))
-    -> {z : Z & can = Nint z # bs = [] # Z.abs_nat z < b}.
-Proof.
-  introv r.
-  unfold subst, lsubst in r; allsimpl; boolvar;
-  repndors; try (subst v'); tcsp;
-  allrw not_over_or; repnd; GC;
-  try (complete (match goal with
-                   | [ H : context[fresh_var ?l] |- _ ] =>
-                     let h := fresh "h" in
-                     pose proof (fresh_var_not_in l) as h;
-                   unfold all_vars in h;
-                   simpl in h;
-                   repeat (rw in_app_iff in h);
-                   repeat (rw not_over_or in h);
-                   repnd; allsimpl; tcsp
-                 end));
-  allsimpl; boolvar; tcsp; fold_terms; allrw app_nil_r.
-
-  { unfold hasvalue_like in r; exrepnd.
-
-    apply reduces_to_split2 in r1; dorn r1; allsimpl; exrepnd; subst.
-
-    { unfold isvalue_like in r0; allsimpl; sp. }
-
-    csunf r1; allsimpl.
-    unfold on_success in r1.
-    csunf r1; allsimpl.
-    dcwf h; allsimpl.
-    unfold compute_step_comp in r1.
-    destruct bs; allsimpl; ginv.
-    remember (get_param_from_cop can) as g; symmetry in Heqg; destruct g; ginv.
-    destruct p; ginv.
-    allapply @get_param_from_cop_pki; subst.
-
-    apply reduces_to_split2 in r2; dorn r2; allsimpl; exrepnd; subst.
-
-    { unfold isvalue_like in r0; allsimpl; sp. }
-
-    boolvar; allsimpl; ginv.
-
-    - apply reduces_to_split2 in r1; repndors; csunf r2; allsimpl; exrepnd; subst; ginv.
-
-      { unfold isvalue_like in r0; allsimpl; sp. }
-
-      csunf r1; allsimpl.
-      dcwf h; allsimpl.
-      unfold compute_step_comp in r1; allsimpl; ginv.
-      boolvar; allsimpl.
-
-      + apply reduces_to_if_isvalue_like in r3; eauto with slow; subst.
-        exists z; dands; auto.
-        apply abs_of_neg; auto.
-
-      + apply reduces_to_vbot_if_isvalue_like in r3; eauto with slow; subst; sp.
-
-    - csunf r2; allsimpl.
-      dcwf h; allsimpl.
-      unfold compute_step_comp in r2; allsimpl; ginv.
-      boolvar; allsimpl.
-
-      + apply reduces_to_if_isvalue_like in r1; eauto with slow; subst.
-        exists z; dands; auto.
-        apply abs_of_pos; auto.
-
-      + apply reduces_to_vbot_if_isvalue_like in r1; eauto with slow; subst; sp.
-  }
-
-  { unfold hasvalue_like in r; exrepnd.
-
-    apply reduces_to_split2 in r1; dorn r1; allsimpl; exrepnd; subst.
-
-    { unfold isvalue_like in r0; allsimpl; sp. }
-
-    csunf r1; allsimpl.
-    unfold on_success in r1.
-    csunf r1; allsimpl.
-    dcwf h; allsimpl.
-    unfold compute_step_comp in r1.
-    destruct bs; allsimpl; ginv.
-    remember (get_param_from_cop can) as g; symmetry in Heqg; destruct g; ginv.
-    destruct p; ginv.
-    allapply @get_param_from_cop_pki; subst.
-
-    apply reduces_to_split2 in r2; dorn r2; allsimpl; exrepnd; subst.
-
-    { unfold isvalue_like in r0; allsimpl; sp. }
-
-    boolvar; allsimpl; ginv.
-
-    - apply reduces_to_split2 in r1; dorn r1; allsimpl; exrepnd; subst; csunf r2; allsimpl; ginv.
-
-      { unfold isvalue_like in r0; allsimpl; sp. }
-
-      csunf r1; allsimpl.
-      dcwf h; allsimpl.
-      unfold compute_step_comp in r1; allsimpl; ginv.
-      boolvar; allsimpl.
-
-      + apply reduces_to_if_isvalue_like in r3; eauto with slow; subst.
-        exists z; dands; auto.
-        apply abs_of_neg; auto.
-
-      + apply reduces_to_vbot_if_isvalue_like in r3; eauto with slow; subst; sp.
-
-    - csunf r2; allsimpl.
-      dcwf h; allsimpl.
-      unfold compute_step_comp in r2; allsimpl; ginv.
-      boolvar; allsimpl.
-
-      + apply reduces_to_if_isvalue_like in r1; eauto with slow; subst.
-        exists z; dands; auto.
-        apply abs_of_pos; auto.
-
-      + apply reduces_to_vbot_if_isvalue_like in r1; eauto with slow; subst; sp.
-  }
-Qed.
-
-Lemma compose_reduces_to_step_primarg_ncompop {o} :
-  forall lib c can bs (t1 t2 u : @NTerm o) l,
-    reduces_to
-      lib
-      (oterm (NCan (NCompOp c))
-             (bterm [] (oterm (Can can) bs) :: bterm [] t1 :: l)) u
-    -> compute_step lib t1 = csuccess t2
-    -> isvalue_like u
-    -> reduces_to
-         lib
-         (oterm (NCan (NCompOp c))
-                (bterm [] (oterm (Can can) bs) :: bterm [] t2 :: l)) u.
-Proof.
-  introv r comp isv.
-  apply reduces_to_split2 in r; dorn r.
-  - subst; allunfold @isvalue_like; allsimpl; sp.
-  - exrepnd.
-    csunf r1; allsimpl.
-    dcwf h; allsimpl.
-    destruct t1 as [v1|f1|op1 bs1]; ginv.
-    dopid op1 as [can1|ncan1|exc1|abs1] Case.
-
-    + Case "Can".
-      csunf comp; allsimpl; ginv.
-      apply compute_step_compop_success_can_can in r1; exrepnd; subst.
-      repndors; exrepnd; subst;
-      allrw @get_param_from_cop_some; subst.
-      * apply (reduces_to_if_split2
-                 _ _ (if Z_lt_le_dec n1 n2 then t1 else t2)); auto.
-      * apply (reduces_to_if_split2
-                 _ _ (if param_kind_deq pk1 pk2 then t1 else t2)); auto.
-        csunf; simpl; dcwf h;
-        unfold compute_step_comp; simpl; allrw @get_param_from_cop_pk2can; auto.
-
-    + Case "NCan".
-      unfold on_success in r1.
-      rw comp in r1; ginv; auto.
-
-    + Case "Exc".
-      csunf comp; allsimpl.
-      ginv; allsimpl; ginv.
-      apply (reduces_to_if_split2 _ _ (oterm Exc bs1)); auto.
-      csunf; simpl; dcwf h; auto.
-
-    + Case "Abs".
-      unfold on_success in r1.
-      rw comp in r1; ginv; auto.
-Qed.
-
-Lemma compose_reduces_to_step_primarg_arithop {o} :
-  forall lib c can bs (t1 t2 u : @NTerm o) l,
-    reduces_to
-      lib
-      (oterm (NCan (NArithOp c))
-             (bterm [] (oterm (Can can) bs) :: bterm [] t1 :: l)) u
-    -> compute_step lib t1 = csuccess t2
-    -> isvalue_like u
-    -> reduces_to
-         lib
-         (oterm (NCan (NArithOp c))
-                (bterm [] (oterm (Can can) bs) :: bterm [] t2 :: l)) u.
-Proof.
-  introv r comp isv.
-  apply reduces_to_split2 in r; dorn r.
-  - subst; allunfold @isvalue_like; allsimpl; sp.
-  - exrepnd.
-    csunf r1; allsimpl.
-    dcwf h.
-    destruct t1 as [v1|f1|op1 bs1]; ginv.
-    dopid op1 as [can1|ncan1|exc1|abs1] Case.
-
-    + Case "Can".
-      csunf comp; allsimpl.
-      allsimpl; ginv.
-      apply compute_step_arithop_success_can_can in r1; exrepnd; subst.
-      allapply @get_param_from_cop_pki; subst.
-      apply (reduces_to_if_split2
-               _ _ (oterm (Can (Nint (get_arith_op c n1 n2))) [])); auto.
-
-    + Case "NCan".
-      unfold on_success in r1.
-      rw comp in r1; ginv; auto.
-
-    + Case "Exc".
-      csunf comp; allsimpl.
-      ginv; allsimpl; ginv.
-      apply (reduces_to_if_split2
-               _ _ (oterm Exc bs1)); auto.
-      csunf; simpl; dcwf h; auto.
-
-    + Case "Abs".
-      unfold on_success in r1.
-      rw comp in r1; ginv; auto.
-Qed.
-
-Lemma compose_reduces_to_primarg_ncompop {o} :
-  forall lib c can bs (t1 t2 u : @NTerm o) l,
-    reduces_to
-      lib
-      (oterm (NCan (NCompOp c))
-             (bterm [] (oterm (Can can) bs) :: bterm [] t1 :: l)) u
-    -> reduces_to lib t1 t2
-    -> isvalue_like u
-    -> reduces_to
-         lib
-         (oterm (NCan (NCompOp c))
-                (bterm [] (oterm (Can can) bs) :: bterm [] t2 :: l)) u.
-Proof.
-  introv r1 r2 isv.
-  unfold reduces_to in r2; exrepnd.
-  revert dependent t2.
-  revert dependent t1.
-  induction k; introv r1 r2.
-
-  - allrw @reduces_in_atmost_k_steps_0; subst; auto.
-
-  - allrw @reduces_in_atmost_k_steps_S; exrepnd.
-    eapply compose_reduces_to_step_primarg_ncompop in r1;[|eauto|]; auto.
-    eapply IHk; eauto.
-Qed.
-
-Lemma compose_reduces_to_primarg_arithop {o} :
-  forall lib c can bs (t1 t2 u : @NTerm o) l,
-    reduces_to
-      lib
-      (oterm (NCan (NArithOp c))
-             (bterm [] (oterm (Can can) bs) :: bterm [] t1 :: l)) u
-    -> reduces_to lib t1 t2
-    -> isvalue_like u
-    -> reduces_to
-         lib
-         (oterm (NCan (NArithOp c))
-                (bterm [] (oterm (Can can) bs) :: bterm [] t2 :: l)) u.
-Proof.
-  introv r1 r2 isv.
-  unfold reduces_to in r2; exrepnd.
-  revert dependent t2.
-  revert dependent t1.
-  induction k; introv r1 r2.
-
-  - allrw @reduces_in_atmost_k_steps_0; subst; auto.
-
-  - allrw @reduces_in_atmost_k_steps_S; exrepnd.
-    eapply compose_reduces_to_step_primarg_arithop in r1;[|eauto|]; auto.
-    eapply IHk; eauto.
-Qed.
-
-Lemma if_has_value_like_except_ncompop_can1 {o} :
-  forall lib a c can bs (t : @NTerm o) l,
-    has_value_like_except
-      lib a
-      (oterm (NCan (NCompOp c))
-             (bterm [] (oterm (Can can) bs)
-                    :: bterm [] t
-                    :: l))
-    -> has_value_like_except lib a t.
-Proof.
-  introv hv.
-  unfold has_value_like_except in hv; exrepnd.
-
-  pose proof (converges_to_value_like_ncompop lib c can bs t l) as h.
-  autodimp h hyp.
-
-  { unfold converges_to_value_like; exists u; sp. }
-
-  repndors; exrepnd.
-
-  - exists (pk2term pk); dands; eauto 3 with slow.
-    rw @pk2term_eq; simpl; tcsp.
-
-  - exists e; dands; auto.
-    + unfold isvalue_like; simpl; sp.
-    + apply isexc_implies2 in h0; exrepnd; subst.
-      eapply compose_reduces_to_primarg_ncompop in h1; eauto.
-      apply reduces_to_split2 in h1; dorn h1.
-      * subst; allunfold @isvalue_like; allsimpl; sp.
-      * exrepnd; csunf h1; simpl in h1; ginv.
-        dcwf h; ginv.
-        apply reduces_to_if_isvalue_like in h0; eauto with slow.
-        subst; auto.
-Qed.
-
-Lemma if_has_value_like_except_arithop_can1 {o} :
-  forall lib a c can bs (t : @NTerm o) l,
-    has_value_like_except
-      lib a
-      (oterm (NCan (NArithOp c))
-             (bterm [] (oterm (Can can) bs)
-                    :: bterm [] t
-                    :: l))
-    -> has_value_like_except lib a t.
-Proof.
-  introv hv.
-  unfold has_value_like_except in hv; exrepnd.
-
-  pose proof (converges_to_value_like_narithop lib c can bs t l) as h.
-  autodimp h hyp.
-
-  { unfold converges_to_value_like; exists u; sp. }
-
-  repndors; exrepnd.
-
-  - exists (@mk_integer o i); dands.
-    + unfold computes_to_value in h0; sp.
-    + unfold isvalue_like; simpl; sp.
-    + intro k; inversion k.
-
-  - exists e; dands; auto.
-    + unfold isvalue_like; simpl; sp.
-    + apply isexc_implies2 in h0; exrepnd; subst.
-      eapply compose_reduces_to_primarg_arithop in h1; eauto.
-      apply reduces_to_split2 in h1; dorn h1.
-      * subst; allunfold @isvalue_like; allsimpl; sp.
-      * exrepnd; csunf h1; simpl in h1; ginv.
-        dcwf h; ginv.
-        apply reduces_to_if_isvalue_like in h0; eauto with slow.
-        subst; auto.
-Qed.
-
-Lemma if_hasvalue_like_ncompop_can1 {o} :
-  forall lib c can bs (t : @NTerm o) l,
-    hasvalue_like
-      lib
-      (oterm (NCan (NCompOp c))
-             (bterm [] (oterm (Can can) bs)
-                    :: bterm [] t
-                    :: l))
-    -> hasvalue_like lib t.
-Proof.
-  introv hv.
-  unfold hasvalue_like in hv; exrepnd.
-
-  pose proof (converges_to_value_like_ncompop lib c can bs t l) as h.
-  autodimp h hyp.
-
-  { unfold converges_to_value_like; exists v; sp. }
-
-  repndors; exrepnd.
-
-  - exists (pk2term pk); dands; eauto 3 with slow.
-
-  - exists e; dands; auto.
-    unfold isvalue_like; simpl; sp.
-Qed.
-
-Lemma if_hasvalue_like_arithop_can1 {o} :
-  forall lib c can bs (t : @NTerm o) l,
-    hasvalue_like
-      lib
-      (oterm (NCan (NArithOp c))
-             (bterm [] (oterm (Can can) bs)
-                    :: bterm [] t
-                    :: l))
-    -> hasvalue_like lib t.
-Proof.
-  introv hv.
-  unfold has_value_like_except in hv; exrepnd.
-
-  pose proof (converges_to_value_like_narithop lib c can bs t l) as h.
-  autodimp h hyp.
-
-  repndors; exrepnd.
-
-  - exists (@mk_integer o i); dands.
-    + unfold computes_to_value in h0; sp.
-    + unfold isvalue_like; simpl; sp.
-
-  - exists e; dands; auto.
-    unfold isvalue_like; simpl; sp.
-Qed.
-
-Lemma reduces_in_atmost_k_steps_if_isvalue_like {o} :
-  forall lib k (t1 t2 : @NTerm o),
-    reduces_in_atmost_k_steps lib t1 t2 k
-    -> isvalue_like t1
-    -> t2 = t1.
-Proof.
-  induction k; introv r iv.
-  - rw @reduces_in_atmost_k_steps_0 in r; auto.
-  - rw @reduces_in_atmost_k_steps_S in r; exrepnd.
-    rw @compute_step_value_like in r1; auto; ginv.
-    apply IHk in r0; auto; subst; auto.
-Qed.
-
-Lemma reduces_in_atmost_k_steps_if_reduces_to {o} :
-  forall lib k (t1 t2 v : @NTerm o),
-    reduces_in_atmost_k_steps lib t1 v k
-    -> reduces_to lib t1 t2
-    -> isvalue_like v
-    -> {k' : nat & k' <= k # reduces_in_atmost_k_steps lib t2 v k'}.
-Proof.
-  introv r1 r2 iv.
-  unfold reduces_to in r2; exrepnd.
-  destruct (le_gt_dec k0 k) as [i|i].
-  - pose proof (reduces_atmost_split lib k0 k t1 t2 v) as h.
-    repeat (autodimp h hyp).
-    exists (k - k0); dands; auto; try omega.
-  - pose proof (reduces_atmost_split lib k k0 t1 v t2) as h.
-    repeat (autodimp h hyp); try omega.
-    apply reduces_in_atmost_k_steps_if_isvalue_like in h; auto; subst.
-    exists 0; dands; auto; try omega.
-    rw @reduces_in_atmost_k_steps_0; auto.
-Qed.
-
 Lemma wf_term_absolute_value {o} :
   forall (t : @NTerm o), wf_term (absolute_value t) <=> wf_term t.
 Proof.
@@ -1596,47 +271,6 @@ Proof.
   - left.
     exists i1.
     split; eauto 3 with slow.
-Qed.
-
-Lemma computes_to_exception_minus {o} :
-  forall lib (t : @NTerm o) a e,
-    wf_term t
-    -> computes_to_exception lib a (mk_minus t) e
-    -> computes_to_exception lib a t e.
-Proof.
-  introv wf r.
-  allunfold @computes_to_exception.
-  unfold reduces_to in r; exrepnd.
-  revert dependent t.
-  induction k; introv wf comp.
-
-  - allrw @reduces_in_atmost_k_steps_0; ginv.
-
-  - allrw @reduces_in_atmost_k_steps_S; exrepnd.
-
-    csunf comp1; allsimpl.
-    destruct t as [v|f|op bs]; ginv.
-    dopid op as [can|ncan|exc|abs] Case; allsimpl; ginv.
-
-    + Case "Can".
-      apply compute_step_minus_success in comp1; exrepnd; subst; GC; fold_terms.
-      apply computation3.reduces_in_atmost_k_steps_if_isvalue_like in comp0; eauto 3 with slow; ginv.
-
-    + Case "NCan".
-      remember (compute_step lib (oterm (NCan ncan) bs)) as cs; symmetry in Heqcs; destruct cs; allsimpl; ginv.
-      applydup @compute_step_preserves_wf in Heqcs; auto.
-      apply IHk in comp0; auto.
-      eapply reduces_to_if_split2; eauto.
-
-    + Case "Exc".
-      apply computation3.reduces_in_atmost_k_steps_if_isvalue_like in comp0; eauto 3 with slow; ginv.
-      unfold mk_exception in comp0; ginv; eauto 3 with slow.
-
-    + Case "Abs".
-      remember (compute_step lib (oterm (Abs abs) bs)) as cs; symmetry in Heqcs; destruct cs; allsimpl; ginv.
-      applydup @compute_step_preserves_wf in Heqcs; auto.
-      apply IHk in comp0; auto.
-      eapply reduces_to_if_split2; eauto.
 Qed.
 
 Lemma computes_to_exception_absolute_value {o} :
@@ -1872,6 +506,182 @@ XXXXXXXXXXXX
   }
 Qed.
  *)
+
+Lemma hasvalue_like_subst_less_bound {o} :
+  forall lib b v can (bs : list (@BTerm o)),
+    hasvalue_like
+      lib
+      (subst (less_bound b (mk_var v) (mk_vbot v)) v (oterm (Can can) bs))
+    -> {z : Z & can = Nint z # bs = [] # Z.abs_nat z < b}.
+Proof.
+  introv r.
+  unfold subst, lsubst in r; allsimpl; boolvar;
+  repndors; try (subst v'); tcsp;
+  allrw not_over_or; repnd; GC;
+  try (complete (match goal with
+                   | [ H : context[fresh_var ?l] |- _ ] =>
+                     let h := fresh "h" in
+                     pose proof (fresh_var_not_in l) as h;
+                   unfold all_vars in h;
+                   simpl in h;
+                   repeat (rw in_app_iff in h);
+                   repeat (rw not_over_or in h);
+                   repnd; allsimpl; tcsp
+                 end));
+  allsimpl; boolvar; tcsp; fold_terms; allrw app_nil_r.
+
+  { unfold hasvalue_like in r; exrepnd.
+
+    apply reduces_to_split2 in r1; dorn r1; allsimpl; exrepnd; subst.
+
+    { unfold isvalue_like in r0; allsimpl; sp. }
+
+    csunf r1; allsimpl.
+    unfold on_success in r1.
+    csunf r1; allsimpl.
+    dcwf h; allsimpl.
+    unfold compute_step_comp in r1.
+    destruct bs; allsimpl; ginv.
+    remember (get_param_from_cop can) as g; symmetry in Heqg; destruct g; ginv.
+    destruct p; ginv.
+    allapply @get_param_from_cop_pki; subst.
+
+    apply reduces_to_split2 in r2; dorn r2; allsimpl; exrepnd; subst.
+
+    { unfold isvalue_like in r0; allsimpl; sp. }
+
+    boolvar; allsimpl; ginv.
+
+    - apply reduces_to_split2 in r1; repndors; csunf r2; allsimpl; exrepnd; subst; ginv.
+
+      { unfold isvalue_like in r0; allsimpl; sp. }
+
+      csunf r1; allsimpl.
+      dcwf h; allsimpl.
+      unfold compute_step_comp in r1; allsimpl; ginv.
+      boolvar; allsimpl.
+
+      + apply reduces_to_if_isvalue_like in r3; eauto with slow; subst.
+        exists z; dands; auto.
+        apply abs_of_neg; auto.
+
+      + apply reduces_to_vbot_if_isvalue_like in r3; eauto with slow; subst; sp.
+
+    - csunf r2; allsimpl.
+      dcwf h; allsimpl.
+      unfold compute_step_comp in r2; allsimpl; ginv.
+      boolvar; allsimpl.
+
+      + apply reduces_to_if_isvalue_like in r1; eauto with slow; subst.
+        exists z; dands; auto.
+        apply abs_of_pos; auto.
+
+      + apply reduces_to_vbot_if_isvalue_like in r1; eauto with slow; subst; sp.
+  }
+
+  { unfold hasvalue_like in r; exrepnd.
+
+    apply reduces_to_split2 in r1; dorn r1; allsimpl; exrepnd; subst.
+
+    { unfold isvalue_like in r0; allsimpl; sp. }
+
+    csunf r1; allsimpl.
+    unfold on_success in r1.
+    csunf r1; allsimpl.
+    dcwf h; allsimpl.
+    unfold compute_step_comp in r1.
+    destruct bs; allsimpl; ginv.
+    remember (get_param_from_cop can) as g; symmetry in Heqg; destruct g; ginv.
+    destruct p; ginv.
+    allapply @get_param_from_cop_pki; subst.
+
+    apply reduces_to_split2 in r2; dorn r2; allsimpl; exrepnd; subst.
+
+    { unfold isvalue_like in r0; allsimpl; sp. }
+
+    boolvar; allsimpl; ginv.
+
+    - apply reduces_to_split2 in r1; dorn r1; allsimpl; exrepnd; subst; csunf r2; allsimpl; ginv.
+
+      { unfold isvalue_like in r0; allsimpl; sp. }
+
+      csunf r1; allsimpl.
+      dcwf h; allsimpl.
+      unfold compute_step_comp in r1; allsimpl; ginv.
+      boolvar; allsimpl.
+
+      + apply reduces_to_if_isvalue_like in r3; eauto with slow; subst.
+        exists z; dands; auto.
+        apply abs_of_neg; auto.
+
+      + apply reduces_to_vbot_if_isvalue_like in r3; eauto with slow; subst; sp.
+
+    - csunf r2; allsimpl.
+      dcwf h; allsimpl.
+      unfold compute_step_comp in r2; allsimpl; ginv.
+      boolvar; allsimpl.
+
+      + apply reduces_to_if_isvalue_like in r1; eauto with slow; subst.
+        exists z; dands; auto.
+        apply abs_of_pos; auto.
+
+      + apply reduces_to_vbot_if_isvalue_like in r1; eauto with slow; subst; sp.
+  }
+Qed.
+
+Lemma if_hasvalue_like_ncan_primarg {o} :
+  forall lib ncan (t : @NTerm o) bs,
+    hasvalue_like lib (oterm (NCan ncan) (bterm [] t :: bs))
+    -> hasvalue_like lib t.
+Proof.
+  introv hv.
+  allunfold @hasvalue_like; exrepnd.
+  unfold reduces_to in hv1; exrepnd.
+  revert dependent t.
+  induction k; introv r.
+
+  - allrw @reduces_in_atmost_k_steps_0; subst.
+    unfold isvalue_like in hv0; allsimpl; sp.
+
+  - allrw @reduces_in_atmost_k_steps_S; exrepnd.
+    destruct t as [x|f|op l].
+
+    { simpl in r1; ginv. }
+
+    { exists (sterm f); dands; eauto 3 with slow. }
+
+    dopid op as [can1|ncan1|exc1|abs1] Case.
+
+    + Case "Can".
+      exists (oterm (Can can1) l); dands; simpl; eauto with slow; tcsp.
+
+    + Case "NCan".
+      rw @compute_step_ncan_ncan in r1.
+      remember (compute_step lib (oterm (NCan ncan1) l)) as comp.
+      symmetry in Heqcomp; destruct comp; ginv.
+      apply IHk in r0; exrepnd.
+      exists v0; dands; eauto with slow.
+      eapply reduces_to_if_split2; eauto.
+
+    + Case "Exc".
+      csunf r1; allsimpl.
+      apply compute_step_catch_success in r1.
+      dorn r1; exrepnd; subst; allsimpl.
+
+      * exists (oterm Exc [bterm [] a', bterm [] e]); dands; eauto with slow.
+
+      * apply reduces_in_atmost_k_steps_if_isvalue_like in r0; eauto with slow; subst.
+
+    + Case "Abs".
+      csunf r1; allsimpl.
+      csunf r1; allsimpl.
+      unfold on_success in r1.
+      remember (compute_step_lib lib abs1 l) as comp.
+      symmetry in Heqcomp; destruct comp; ginv.
+      apply IHk in r0; exrepnd.
+      exists v0; dands; eauto with slow.
+      eapply reduces_to_if_split2; eauto.
+Qed.
 
 Lemma hasvalue_like_subst_less_bound_seq {o} :
   forall lib b v e (f : @ntseq o),
@@ -2272,6 +1082,12 @@ Proof.
         eapply reduces_to_if_split2; eauto.
 Qed.
 
+Definition has_value_like_except {p} lib a (t : @NTerm p) :=
+  {u : NTerm
+   & reduces_to lib t u
+   # isvalue_like u
+   # !isnexc lib a u}.
+
 Lemma if_has_value_like_except_force_int_bound {o} :
   forall lib a v b (t : @NTerm o),
     nt_wf t
@@ -2331,65 +1147,426 @@ Proof.
   - exists v0; dands; eauto with slow.
 Qed.
 
-Lemma reduces_to_cbv_to_value_like {o} :
-  forall lib (t : @NTerm o) v b u,
-    reduces_to lib (mk_cbv t v b) u
-    -> isvalue_like u
-    -> {c : NTerm & reduces_to lib t c # iscan c # reduces_to lib (subst b v c) u}
-       [+]
-       (reduces_to lib t u # isexc u).
+(*
+Lemma if_has_value_like_except_ncan_primarg {o} :
+  forall lib a ncan (t : @NTerm o) bs,
+    has_value_like_except lib a (oterm (NCan ncan) (bterm [] t :: bs))
+    -> has_value_like_except lib a t.
 Proof.
-  introv r.
-  unfold reduces_to in r; exrepnd.
+  introv hv.
+  allunfold @has_value_like_except; exrepnd.
+  unfold reduces_to in hv1; exrepnd.
   revert dependent t.
-  induction k; introv r isv.
+  induction k; introv r.
 
   - allrw @reduces_in_atmost_k_steps_0; subst.
-    unfold isvalue_like in isv; allsimpl; sp.
+    unfold isvalue_like in hv2; allsimpl; sp.
 
   - allrw @reduces_in_atmost_k_steps_S; exrepnd.
-    destruct t as [x|f|op bs]; try (complete (allsimpl; ginv)).
+    destruct t as [v|op l].
 
-    { csunf r1; allsimpl; ginv.
-      allunfold @apply_bterm; allsimpl; allrw @fold_subst.
-      left.
-      exists (sterm f); simpl; dands; eauto 3 with slow. }
+    { simpl in r1; ginv. }
 
-    dopid op as [can|ncan|exc|abs] Case.
+    dopid op as [can1|ncan1|exc1|abs1] Case.
 
     + Case "Can".
-      csunf r1; simpl in r1; ginv.
-      left.
-      unfold apply_bterm in r0; allsimpl.
-      exists (oterm (Can can) bs); dands; eauto with slow.
+      exists (oterm (Can can1) l); dands; simpl; eauto with slow; tcsp.
 
     + Case "NCan".
-      rw @compute_step_cbv_ncan in r1.
-      remember (compute_step lib (oterm (NCan ncan) bs)) as comp.
+      rw @compute_step_ncan_ncan in r1.
+      remember (compute_step lib (oterm (NCan ncan1) l)) as comp.
       symmetry in Heqcomp; destruct comp; ginv.
-      apply IHk in r0; auto; dorn r0; exrepnd.
-
-      * left; exists c; dands; eauto with slow.
-        eapply reduces_to_if_split2; eauto.
-
-      * right; dands; eauto with slow.
-        eapply reduces_to_if_split2; eauto.
+      apply IHk in r0; exrepnd.
+      exists u0; dands; eauto with slow.
+      eapply reduces_to_if_split2; eauto.
 
     + Case "Exc".
-      csunf r1; allsimpl; ginv.
-      apply reduces_in_atmost_k_steps_if_isvalue_like in r0; subst; eauto with slow.
+      csunf r1; allsimpl.
+      apply compute_step_catch_success in r1.
+      repndors; exrepnd; subst; allsimpl.
+
+      *
+
+Lemma reduces_in_atmost_k_steps_mk_atom_eq {o}:
+  forall lib (a b c d : @NTerm o) u,
+    reduces_in_atmost_k_steps lib (mk_atom_eq a b c d) u k
+    -> isvalue_like u
+    -> {k1 : nat
+        & {k2 : nat
+        & {v1 : NTerm
+        & {v2 : NTerm
+        & reduces_in_atmost_k_steps lib a v1 k1
+        # reduces_in_atmost_k_steps lib b v2 k2
+        # }}}}.
+Proof.
+Qed.
+
+        exists (oterm Exc [bterm [] a', bterm [] e]); dands; eauto with slow.
+        allsimpl.
+        destruct exc1; allsimpl; tcsp.
+        boolvar; ginv; allrw not_over_or; tcsp.
+
+      * apply reduces_in_atmost_k_steps_if_isvalue_like in r0; eauto with slow; subst.
+        exists (oterm (Exc exc1) l); dands; eauto with slow.
+
+    + Case "Mrk".
+      allsimpl; ginv.
+      apply reduces_in_atmost_k_steps_primarg_marker in r0; subst.
+      unfold isvalue_like in hv2; allsimpl; sp.
 
     + Case "Abs".
-      rw @compute_step_cbv_abs in r1.
-      remember (compute_step lib (oterm (Abs abs) bs)) as comp.
+      allsimpl.
+      unfold on_success in r1.
+      remember (compute_step_lib lib abs1 l) as comp.
       symmetry in Heqcomp; destruct comp; ginv.
-      apply IHk in r0; auto; dorn r0; exrepnd.
+      apply IHk in r0; exrepnd.
+      exists u0; dands; eauto with slow.
+      eapply reduces_to_if_split2; eauto.
+Qed.
+*)
 
-      * left; exists c; dands; eauto with slow.
-        eapply reduces_to_if_split2; eauto.
+(*
+Lemma if_has_value_like_except_exc {o} :
+  forall lib a exc (bs : list (@BTerm o)),
+    has_value_like_except lib a (oterm (Exc exc) bs)
+    -> exc <> Some a.
+Proof.
+  introv hv.
+  unfold has_value_like_except in hv; exrepnd.
+  apply reduces_to_if_isvalue_like in hv1; eauto with slow.
+  subst.
+  introv k.
+  destruct exc; allsimpl; ginv; boolvar; cpx.
+Qed.
+*)
 
-      * right; dands; eauto with slow.
-        eapply reduces_to_if_split2; eauto.
+(*
+Lemma compute_step_apply_failure {o} :
+  forall can (bs1 bs2 : list (@BTerm o)) s t,
+    compute_step_apply
+      can
+      (oterm (NCan NApply) (bterm [] (oterm (Can can) bs1) :: bs2))
+      bs1 bs2 = cfailure s t
+    -> (
+         (can = NLambda
+          # (forall v b, bs1 <> [bterm [v] b])
+          # s = compute_step_apply_not_well_formed
+          # t = oterm (NCan NApply) (bterm [] (oterm (Can can) bs1) :: bs2))
+         [+]
+         (can = NLambda
+          # (forall arg, bs2 <> [bterm [] arg])
+          # s = compute_step_apply_not_well_formed
+          # t = oterm (NCan NApply) (bterm [] (oterm (Can can) bs1) :: bs2))
+         [+]
+         (can <> NLambda
+          # s = bad_first_arg
+          # t = oterm (NCan NApply) (bterm [] (oterm (Can can) bs1) :: bs2))
+       ).
+Proof.
+  introv comp.
+  destruct can;
+    try (complete (simpl in comp; ginv; right; right; dands; tcsp; intro k; inversion k)).
+  destruct bs1.
+  - simpl in comp; ginv.
+    left; dands; sp.
+  - destruct bs1.
+    + destruct b.
+      destruct l.
+      * simpl in comp; ginv.
+        left; dands; tcsp.
+        introv k; tcsp; ginv.
+      * destruct l.
+        { destruct bs2.
+          { simpl in comp; ginv.
+            right; left; sp. }
+          { destruct bs2.
+            - destruct b.
+              destruct l.
+              + simpl in comp; ginv.
+              + simpl in comp; ginv.
+                right; left; dands; tcsp.
+                introv k; ginv.
+            - destruct b.
+              destruct l.
+              + simpl in comp; ginv.
+                right; left; dands; tcsp.
+              + simpl in comp; ginv.
+                right; left; dands; tcsp.
+          }
+        }
+        { simpl in comp; ginv.
+          left; dands; tcsp.
+          introv k; ginv. }
+    + destruct b.
+      destruct l.
+      * simpl in comp; ginv.
+        left; dands; tcsp.
+      * destruct l.
+        { simpl in comp; ginv.
+          left; dands; tcsp. }
+        { simpl in comp; ginv.
+          left; dands; tcsp. }
+Qed.
+*)
+
+Lemma wf_force_int_bound {o} :
+  forall v b (t : @NTerm o) e,
+    wf_term (force_int_bound v b t e) <=> (wf_term t # wf_term e).
+Proof.
+  introv.
+  unfold force_int_bound.
+  rw <- @wf_cbv_iff.
+  unfold less_bound.
+  rw <- @wf_less_iff.
+  unfold absolute_value.
+  rw <- @wf_less_iff.
+  rw <- @wf_minus_iff.
+  split; introv k; repndors; repnd; dands; tcsp.
+Qed.
+
+Lemma wf_term_force_int_bound_F_if {o} :
+  forall x b (F f e : @NTerm o),
+    wf_term F
+    -> wf_term f
+    -> wf_term e
+    -> wf_term (force_int_bound_F x b F f e).
+Proof.
+  introv wF wf we.
+  unfold force_int_bound_F.
+  apply wf_apply; auto.
+  unfold force_int_bound_f.
+  apply wf_lam.
+  apply wf_cbv.
+  - apply wf_force_int_bound; sp.
+  - apply wf_apply; sp.
+Qed.
+Hint Resolve wf_term_force_int_bound_F_if : slow.
+
+Lemma wf_term_force_int_F_if {o} :
+  forall x (F f : @NTerm o),
+    wf_term F
+    -> wf_term f
+    -> wf_term (force_int_F x F f).
+Proof.
+  introv wF wf.
+  unfold force_int_F.
+  apply wf_apply; auto.
+  unfold force_int_f.
+  apply wf_lam.
+  apply wf_cbv; tcsp.
+  apply wf_apply; sp.
+Qed.
+Hint Resolve wf_term_force_int_F_if : slow.
+
+Lemma reduces_to_int_subst_less_bound {o} :
+  forall lib b v a can z (bs : list (@BTerm o)),
+    reduces_to
+      lib
+      (subst (less_bound b (mk_var v) (uexc a)) v (oterm (Can can) bs))
+      (mk_integer z)
+    -> can = Nint z # bs = [] # Z.abs_nat z < b.
+Proof.
+  introv r.
+  unfold subst, lsubst in r; allsimpl; boolvar.
+  fold_terms.
+
+  apply reduces_to_split2 in r; dorn r; allsimpl; exrepnd; ginv.
+  csunf r1; allsimpl.
+  unfold on_success in r1.
+  csunf r1; allsimpl.
+  dcwf h; allsimpl.
+  unfold compute_step_comp in r1.
+  destruct bs; allsimpl; ginv.
+  remember (get_param_from_cop can) as g; symmetry in Heqg; destruct g; ginv.
+  destruct p; ginv.
+  allapply @get_param_from_cop_pki; subst.
+
+  apply reduces_to_split2 in r0; dorn r0; allsimpl; exrepnd; ginv.
+  csunf r0; allsimpl.
+  boolvar; allsimpl; ginv.
+
+  - apply reduces_to_split2 in r1; dorn r1; ginv.
+    exrepnd; allsimpl.
+    csunf r1; allsimpl.
+    dcwf h; allsimpl.
+    unfold compute_step_comp in r1; allsimpl; ginv.
+    boolvar; allsimpl.
+
+    + apply reduces_to_if_isvalue_like in r0; eauto with slow.
+      inversion r0; subst; dands; auto.
+      apply abs_of_neg; auto.
+
+    + apply reduces_to_if_isvalue_like in r0; eauto with slow.
+      inversion r0.
+
+  - dcwf h; allsimpl.
+    unfold compute_step_comp in r0; allsimpl; ginv.
+    boolvar; allsimpl.
+
+    + apply reduces_to_if_isvalue_like in r1; eauto with slow.
+      inversion r1; subst; dands; auto.
+      apply abs_of_pos; auto.
+
+    + apply reduces_to_if_isvalue_like in r1; eauto with slow.
+      inversion r1.
+Qed.
+
+Lemma has_value_like_except_subst_less_bound {o} :
+  forall lib b v a can (bs : list (@BTerm o)),
+    has_value_like_except
+      lib a
+      (subst (less_bound b (mk_var v) (uexc a)) v (oterm (Can can) bs))
+    -> {z : Z & can = Nint z # bs = [] # Z.abs_nat z < b}.
+Proof.
+  introv r.
+  unfold subst, lsubst in r; allsimpl; boolvar.
+  fold_terms.
+  unfold has_value_like_except in r; exrepnd.
+
+  apply reduces_to_split2 in r1; dorn r1; allsimpl; exrepnd; subst.
+
+  { unfold isvalue_like in r2; exrepnd; repndors; inversion r2. }
+
+  csunf r1; allsimpl.
+  unfold on_success in r1.
+  csunf r1; allsimpl.
+  dcwf h; allsimpl.
+  unfold compute_step_comp in r1.
+  destruct bs; allsimpl; ginv.
+  remember (get_param_from_cop can) as g; symmetry in Heqg; destruct g; ginv.
+  destruct p; ginv.
+  allapply @get_param_from_cop_pki; subst.
+
+  apply reduces_to_split2 in r3; dorn r3; allsimpl; exrepnd; subst.
+
+  { unfold isvalue_like in r2; exrepnd; repndors; inversion r2. }
+
+  csunf r3; allsimpl; boolvar; allsimpl; ginv.
+
+  - apply reduces_to_split2 in r1; dorn r1; allsimpl; exrepnd; subst.
+
+    { unfold isvalue_like in r2; exrepnd; repndors; inversion r2. }
+
+    csunf r1; allsimpl.
+    dcwf h; allsimpl.
+    unfold compute_step_comp in r1; allsimpl; ginv.
+    boolvar; allsimpl.
+
+    + apply reduces_to_if_isvalue_like in r3; eauto with slow; subst.
+      exists z; dands; auto.
+      apply abs_of_neg; auto.
+
+    + apply reduces_to_if_isvalue_like in r3; eauto with slow; subst.
+      destruct r0; simpl; exists (mk_utoken a); simpl; boolvar; dands; tcsp; eauto with slow.
+
+  - dcwf h; allsimpl.
+    unfold compute_step_comp in r3; allsimpl; ginv.
+    boolvar; allsimpl.
+
+    + apply reduces_to_if_isvalue_like in r1; eauto with slow; subst.
+      exists z; dands; auto.
+      apply abs_of_pos; auto.
+
+    + apply reduces_to_if_isvalue_like in r1; eauto with slow; subst.
+      destruct r0; simpl; exists (mk_utoken a); simpl; boolvar; dands; tcsp; eauto with slow.
+Qed.
+
+Lemma if_has_value_like_except_ncompop_can1 {o} :
+  forall lib a c can bs (t : @NTerm o) l,
+    has_value_like_except
+      lib a
+      (oterm (NCan (NCompOp c))
+             (bterm [] (oterm (Can can) bs)
+                    :: bterm [] t
+                    :: l))
+    -> has_value_like_except lib a t.
+Proof.
+  introv hv.
+  unfold has_value_like_except in hv; exrepnd.
+
+  pose proof (converges_to_value_like_ncompop lib c can bs t l) as h.
+  autodimp h hyp.
+
+  { unfold converges_to_value_like; exists u; sp. }
+
+  repndors; exrepnd.
+
+  - exists (pk2term pk); dands; eauto 3 with slow.
+    rw @pk2term_eq; simpl; tcsp.
+
+  - exists e; dands; auto.
+    + unfold isvalue_like; simpl; sp.
+    + apply isexc_implies2 in h0; exrepnd; subst.
+      eapply compose_reduces_to_primarg_ncompop in h1; eauto.
+      apply reduces_to_split2 in h1; dorn h1.
+      * subst; allunfold @isvalue_like; allsimpl; sp.
+      * exrepnd; csunf h1; simpl in h1; ginv.
+        dcwf h; ginv.
+        apply reduces_to_if_isvalue_like in h0; eauto with slow.
+        subst; auto.
+Qed.
+
+Lemma if_has_value_like_except_arithop_can1 {o} :
+  forall lib a c can bs (t : @NTerm o) l,
+    has_value_like_except
+      lib a
+      (oterm (NCan (NArithOp c))
+             (bterm [] (oterm (Can can) bs)
+                    :: bterm [] t
+                    :: l))
+    -> has_value_like_except lib a t.
+Proof.
+  introv hv.
+  unfold has_value_like_except in hv; exrepnd.
+
+  pose proof (converges_to_value_like_narithop lib c can bs t l) as h.
+  autodimp h hyp.
+
+  { unfold converges_to_value_like; exists u; sp. }
+
+  repndors; exrepnd.
+
+  - exists (@mk_integer o i); dands.
+    + unfold computes_to_value in h0; sp.
+    + unfold isvalue_like; simpl; sp.
+    + intro k; inversion k.
+
+  - exists e; dands; auto.
+    + unfold isvalue_like; simpl; sp.
+    + apply isexc_implies2 in h0; exrepnd; subst.
+      eapply compose_reduces_to_primarg_arithop in h1; eauto.
+      apply reduces_to_split2 in h1; dorn h1.
+      * subst; allunfold @isvalue_like; allsimpl; sp.
+      * exrepnd; csunf h1; simpl in h1; ginv.
+        dcwf h; ginv.
+        apply reduces_to_if_isvalue_like in h0; eauto with slow.
+        subst; auto.
+Qed.
+
+Lemma if_hasvalue_like_arithop_can1 {o} :
+  forall lib c can bs (t : @NTerm o) l,
+    hasvalue_like
+      lib
+      (oterm (NCan (NArithOp c))
+             (bterm [] (oterm (Can can) bs)
+                    :: bterm [] t
+                    :: l))
+    -> hasvalue_like lib t.
+Proof.
+  introv hv.
+  unfold has_value_like_except in hv; exrepnd.
+
+  pose proof (converges_to_value_like_narithop lib c can bs t l) as h.
+  autodimp h hyp.
+
+  repndors; exrepnd.
+
+  - exists (@mk_integer o i); dands.
+    + unfold computes_to_value in h0; sp.
+    + unfold isvalue_like; simpl; sp.
+
+  - exists e; dands; auto.
+    unfold isvalue_like; simpl; sp.
 Qed.
 
 Lemma reduces_to_int_subst_less_bound3 {o} :
@@ -2477,447 +1654,6 @@ Proof.
       autodimp k hyp; try omega.
       allrw Znat.Zabs2Nat.id.
       destruct z; allsimpl; try omega.
-Qed.
-
-(*
-Lemma if_has_value_like_except_ncan_primarg {o} :
-  forall lib a ncan (t : @NTerm o) bs,
-    has_value_like_except lib a (oterm (NCan ncan) (bterm [] t :: bs))
-    -> has_value_like_except lib a t.
-Proof.
-  introv hv.
-  allunfold @has_value_like_except; exrepnd.
-  unfold reduces_to in hv1; exrepnd.
-  revert dependent t.
-  induction k; introv r.
-
-  - allrw @reduces_in_atmost_k_steps_0; subst.
-    unfold isvalue_like in hv2; allsimpl; sp.
-
-  - allrw @reduces_in_atmost_k_steps_S; exrepnd.
-    destruct t as [v|op l].
-
-    { simpl in r1; ginv. }
-
-    dopid op as [can1|ncan1|exc1|abs1] Case.
-
-    + Case "Can".
-      exists (oterm (Can can1) l); dands; simpl; eauto with slow; tcsp.
-
-    + Case "NCan".
-      rw @compute_step_ncan_ncan in r1.
-      remember (compute_step lib (oterm (NCan ncan1) l)) as comp.
-      symmetry in Heqcomp; destruct comp; ginv.
-      apply IHk in r0; exrepnd.
-      exists u0; dands; eauto with slow.
-      eapply reduces_to_if_split2; eauto.
-
-    + Case "Exc".
-      csunf r1; allsimpl.
-      apply compute_step_catch_success in r1.
-      repndors; exrepnd; subst; allsimpl.
-
-      *
-
-Lemma reduces_in_atmost_k_steps_mk_atom_eq {o}:
-  forall lib (a b c d : @NTerm o) u,
-    reduces_in_atmost_k_steps lib (mk_atom_eq a b c d) u k
-    -> isvalue_like u
-    -> {k1 : nat
-        & {k2 : nat
-        & {v1 : NTerm
-        & {v2 : NTerm
-        & reduces_in_atmost_k_steps lib a v1 k1
-        # reduces_in_atmost_k_steps lib b v2 k2
-        # }}}}.
-Proof.
-Qed.
-
-        exists (oterm Exc [bterm [] a', bterm [] e]); dands; eauto with slow.
-        allsimpl.
-        destruct exc1; allsimpl; tcsp.
-        boolvar; ginv; allrw not_over_or; tcsp.
-
-      * apply reduces_in_atmost_k_steps_if_isvalue_like in r0; eauto with slow; subst.
-        exists (oterm (Exc exc1) l); dands; eauto with slow.
-
-    + Case "Mrk".
-      allsimpl; ginv.
-      apply reduces_in_atmost_k_steps_primarg_marker in r0; subst.
-      unfold isvalue_like in hv2; allsimpl; sp.
-
-    + Case "Abs".
-      allsimpl.
-      unfold on_success in r1.
-      remember (compute_step_lib lib abs1 l) as comp.
-      symmetry in Heqcomp; destruct comp; ginv.
-      apply IHk in r0; exrepnd.
-      exists u0; dands; eauto with slow.
-      eapply reduces_to_if_split2; eauto.
-Qed.
-*)
-
-Lemma if_hasvalue_like_ncan_primarg {o} :
-  forall lib ncan (t : @NTerm o) bs,
-    hasvalue_like lib (oterm (NCan ncan) (bterm [] t :: bs))
-    -> hasvalue_like lib t.
-Proof.
-  introv hv.
-  allunfold @hasvalue_like; exrepnd.
-  unfold reduces_to in hv1; exrepnd.
-  revert dependent t.
-  induction k; introv r.
-
-  - allrw @reduces_in_atmost_k_steps_0; subst.
-    unfold isvalue_like in hv0; allsimpl; sp.
-
-  - allrw @reduces_in_atmost_k_steps_S; exrepnd.
-    destruct t as [x|f|op l].
-
-    { simpl in r1; ginv. }
-
-    { exists (sterm f); dands; eauto 3 with slow. }
-
-    dopid op as [can1|ncan1|exc1|abs1] Case.
-
-    + Case "Can".
-      exists (oterm (Can can1) l); dands; simpl; eauto with slow; tcsp.
-
-    + Case "NCan".
-      rw @compute_step_ncan_ncan in r1.
-      remember (compute_step lib (oterm (NCan ncan1) l)) as comp.
-      symmetry in Heqcomp; destruct comp; ginv.
-      apply IHk in r0; exrepnd.
-      exists v0; dands; eauto with slow.
-      eapply reduces_to_if_split2; eauto.
-
-    + Case "Exc".
-      csunf r1; allsimpl.
-      apply compute_step_catch_success in r1.
-      dorn r1; exrepnd; subst; allsimpl.
-
-      * exists (oterm Exc [bterm [] a', bterm [] e]); dands; eauto with slow.
-
-      * apply reduces_in_atmost_k_steps_if_isvalue_like in r0; eauto with slow; subst.
-
-    + Case "Abs".
-      csunf r1; allsimpl.
-      csunf r1; allsimpl.
-      unfold on_success in r1.
-      remember (compute_step_lib lib abs1 l) as comp.
-      symmetry in Heqcomp; destruct comp; ginv.
-      apply IHk in r0; exrepnd.
-      exists v0; dands; eauto with slow.
-      eapply reduces_to_if_split2; eauto.
-Qed.
-
-(*
-Lemma if_has_value_like_except_exc {o} :
-  forall lib a exc (bs : list (@BTerm o)),
-    has_value_like_except lib a (oterm (Exc exc) bs)
-    -> exc <> Some a.
-Proof.
-  introv hv.
-  unfold has_value_like_except in hv; exrepnd.
-  apply reduces_to_if_isvalue_like in hv1; eauto with slow.
-  subst.
-  introv k.
-  destruct exc; allsimpl; ginv; boolvar; cpx.
-Qed.
-*)
-
-(*
-Lemma compute_step_apply_failure {o} :
-  forall can (bs1 bs2 : list (@BTerm o)) s t,
-    compute_step_apply
-      can
-      (oterm (NCan NApply) (bterm [] (oterm (Can can) bs1) :: bs2))
-      bs1 bs2 = cfailure s t
-    -> (
-         (can = NLambda
-          # (forall v b, bs1 <> [bterm [v] b])
-          # s = compute_step_apply_not_well_formed
-          # t = oterm (NCan NApply) (bterm [] (oterm (Can can) bs1) :: bs2))
-         [+]
-         (can = NLambda
-          # (forall arg, bs2 <> [bterm [] arg])
-          # s = compute_step_apply_not_well_formed
-          # t = oterm (NCan NApply) (bterm [] (oterm (Can can) bs1) :: bs2))
-         [+]
-         (can <> NLambda
-          # s = bad_first_arg
-          # t = oterm (NCan NApply) (bterm [] (oterm (Can can) bs1) :: bs2))
-       ).
-Proof.
-  introv comp.
-  destruct can;
-    try (complete (simpl in comp; ginv; right; right; dands; tcsp; intro k; inversion k)).
-  destruct bs1.
-  - simpl in comp; ginv.
-    left; dands; sp.
-  - destruct bs1.
-    + destruct b.
-      destruct l.
-      * simpl in comp; ginv.
-        left; dands; tcsp.
-        introv k; tcsp; ginv.
-      * destruct l.
-        { destruct bs2.
-          { simpl in comp; ginv.
-            right; left; sp. }
-          { destruct bs2.
-            - destruct b.
-              destruct l.
-              + simpl in comp; ginv.
-              + simpl in comp; ginv.
-                right; left; dands; tcsp.
-                introv k; ginv.
-            - destruct b.
-              destruct l.
-              + simpl in comp; ginv.
-                right; left; dands; tcsp.
-              + simpl in comp; ginv.
-                right; left; dands; tcsp.
-          }
-        }
-        { simpl in comp; ginv.
-          left; dands; tcsp.
-          introv k; ginv. }
-    + destruct b.
-      destruct l.
-      * simpl in comp; ginv.
-        left; dands; tcsp.
-      * destruct l.
-        { simpl in comp; ginv.
-          left; dands; tcsp. }
-        { simpl in comp; ginv.
-          left; dands; tcsp. }
-Qed.
-*)
-
-Lemma reduces_to_steps_alpha {o} :
-  forall lib (t1 t2 t : @NTerm o),
-    nt_wf t1
-    -> alpha_eq t1 t2
-    -> reduces_to lib t1 t
-    -> {u : NTerm $ reduces_to lib t2 u # alpha_eq t u}.
-Proof.
-  introv wf aeq r.
-  unfold reduces_to in r; exrepnd.
-  pose proof (reduces_in_atmost_k_steps_alpha lib t1 t2 wf aeq k t r0) as h.
-  exrepnd.
-  exists t2'; dands; auto.
-  exists k; auto.
-Qed.
-
-Lemma alpha_eq_bterms_nil {o} :
-  @alpha_eq_bterms o [] [].
-Proof.
-  unfold alpha_eq_bterms, br_bterms, br_list; simpl; sp.
-Qed.
-Hint Resolve alpha_eq_bterms_nil : slow.
-
-Lemma alpha_eq_bterms_cons_if {o} :
-  forall (b1 b2 : @BTerm o) bs1 bs2,
-    alpha_eq_bterm b1 b2
-    -> alpha_eq_bterms bs1 bs2
-    -> alpha_eq_bterms (b1 :: bs1) (b2 :: bs2).
-Proof.
-  introv aeq1 aeq2.
-  apply alpha_eq_bterms_cons; auto.
-Qed.
-Hint Resolve alpha_eq_bterms_cons_if : slow.
-
-Lemma length_mk_fresh_bterms {o} :
-  forall v (bs : list (@BTerm o)),
-    length (mk_fresh_bterms v bs) = length bs.
-Proof.
-  introv; unfold mk_fresh_bterms.
-  allrw map_length; auto.
-Qed.
-
-Lemma free_vars_subst_utokens_aux_subset {o} :
-  forall (t : @NTerm o) (sub : utok_sub),
-    subset (free_vars (subst_utokens_aux t sub))
-           (free_vars t ++ free_vars_utok_sub sub).
-Proof.
-  introv.
-  rw <- subvars_eq; apply free_vars_subst_utokens_aux.
-Qed.
-
-Lemma wf_force_int_bound {o} :
-  forall v b (t : @NTerm o) e,
-    wf_term (force_int_bound v b t e) <=> (wf_term t # wf_term e).
-Proof.
-  introv.
-  unfold force_int_bound.
-  rw <- @wf_cbv_iff.
-  unfold less_bound.
-  rw <- @wf_less_iff.
-  unfold absolute_value.
-  rw <- @wf_less_iff.
-  rw <- @wf_minus_iff.
-  split; introv k; repndors; repnd; dands; tcsp.
-Qed.
-
-Lemma wf_term_force_int_bound_F_if {o} :
-  forall x b (F f e : @NTerm o),
-    wf_term F
-    -> wf_term f
-    -> wf_term e
-    -> wf_term (force_int_bound_F x b F f e).
-Proof.
-  introv wF wf we.
-  unfold force_int_bound_F.
-  apply wf_apply; auto.
-  unfold force_int_bound_f.
-  apply wf_lam.
-  apply wf_cbv.
-  - apply wf_force_int_bound; sp.
-  - apply wf_apply; sp.
-Qed.
-Hint Resolve wf_term_force_int_bound_F_if : slow.
-
-Lemma wf_term_force_int_F_if {o} :
-  forall x (F f : @NTerm o),
-    wf_term F
-    -> wf_term f
-    -> wf_term (force_int_F x F f).
-Proof.
-  introv wF wf.
-  unfold force_int_F.
-  apply wf_apply; auto.
-  unfold force_int_f.
-  apply wf_lam.
-  apply wf_cbv; tcsp.
-  apply wf_apply; sp.
-Qed.
-Hint Resolve wf_term_force_int_F_if : slow.
-
-Lemma hasvalue_like_fresh_implies {o} :
-  forall lib a v (t : @NTerm o),
-    wf_term t
-    -> !LIn a (get_utokens t)
-    -> hasvalue_like lib (mk_fresh v t)
-    -> hasvalue_like lib (subst t v (mk_utoken a)).
-Proof.
-  introv wt nia hvl.
-  allunfold @hasvalue_like; exrepnd.
-  unfold reduces_to in hvl1; exrepnd.
-  revert dependent v0.
-  revert dependent t.
-  revert dependent a.
-  induction k; introv wt nia r isvl.
-
-  - allrw @reduces_in_atmost_k_steps_0; subst.
-    unfold isvalue_like in isvl; repndors; inversion isvl.
-
-  - allrw @reduces_in_atmost_k_steps_S; exrepnd.
-    apply compute_step_ncan_bterm_cons_success in r1; repnd; subst; GC.
-    repndors; exrepnd; subst; allsimpl; GC.
-    + apply reduces_in_atmost_k_steps_implies_reduces_to in r0.
-      apply reduces_in_atmost_k_step_fresh_id in r0; tcsp.
-    + apply reduces_in_atmost_k_steps_implies_reduces_to in r0.
-      apply reduces_to_if_isvalue_like in r0; eauto 4 with slow.
-    + repnd; subst.
-      pose proof (compute_step_subst_utoken lib t x [(v,mk_utoken (get_fresh_atom t))]) as h.
-      allrw @get_utokens_sub_cons; allrw @get_utokens_sub_nil; allsimpl.
-      allrw disjoint_singleton_l.
-      repeat (autodimp h hyp); try (apply get_fresh_atom_prop); eauto 3 with slow.
-      { apply nr_ut_sub_cons; eauto 3 with slow.
-        intro i; apply get_fresh_atom_prop. }
-      exrepnd.
-      pose proof (h0 [(v,mk_utoken a)]) as q; clear h0; allsimpl.
-      allrw @get_utokens_sub_cons; allrw @get_utokens_sub_nil; allsimpl.
-      allrw disjoint_singleton_l.
-      repeat (autodimp q hyp); exrepnd.
-      allrw @fold_subst.
-
-      assert (wf_term x) as wfx.
-      { eapply compute_step_preserves_wf;[exact r3|].
-        apply wf_term_subst; eauto with slow. }
-
-      assert (!LIn v (free_vars x)) as nivx.
-      { intro j; apply compute_step_preserves in r3; repnd;
-        [|apply nt_wf_subst; eauto 3 with slow].
-        rw subvars_prop in r2; apply r2 in j; clear r2.
-        apply eqset_free_vars_disjoint in j; allsimpl.
-        allrw in_app_iff; allrw in_remove_nvars; allsimpl; boolvar; allsimpl; tcsp. }
-
-      pose proof (IHk a (subst_utokens x [(get_fresh_atom t, mk_var v)])) as q; clear IHk.
-      repeat (autodimp q hyp).
-      { apply wf_subst_utokens; eauto 3 with slow. }
-      { intro j; apply get_utokens_subst_utokens_subset in j; allsimpl.
-        unfold get_utokens_utok_ren in j; allsimpl; allrw app_nil_r.
-        rw in_remove in j; repnd.
-        apply alphaeq_preserves_utokens in h1; rw h1 in j.
-        apply get_utokens_subst in j; boolvar; allsimpl; allrw in_app_iff; tcsp; allsimpl.
-        repndors; tcsp. }
-
-      pose proof (q v0) as ih; clear q.
-      repeat (autodimp ih hyp); exrepnd.
-
-      pose proof (simple_subst_subst_utokens_aeq x (get_fresh_atom t) v) as aeq1.
-      repeat (autodimp aeq1 hyp).
-
-      pose proof (alpha_eq_ren_utokens
-                    (subst (subst_utokens x [(get_fresh_atom t, mk_var v)]) v
-                           (mk_utoken (get_fresh_atom t)))
-                    x [(get_fresh_atom t, a)] aeq1) as aeq2.
-      rw @subst_ren_utokens in aeq2; allsimpl; fold_terms.
-      unfold ren_atom in aeq2; allsimpl; boolvar; tcsp.
-      rw @ren_utokens_trivial in aeq2;
-        [|simpl; apply disjoint_singleton_l; intro i;
-          apply get_utokens_subst_utokens_subset in i; allsimpl;
-          unfold get_utokens_utok_ren in i; allsimpl; rw app_nil_r in i;
-          rw in_remove in i; repnd; GC;
-          apply alphaeq_preserves_utokens in h1; rw h1 in i;
-          apply get_utokens_subst in i; allsimpl; boolvar; allrw app_nil_r;
-          allrw in_app_iff; repndors; tcsp].
-
-      clear aeq1.
-
-      pose proof (alpha_eq_ren_utokens
-                    x (subst w v (mk_utoken (get_fresh_atom t)))
-                    [(get_fresh_atom t, a)] h1) as aeq3.
-      rw @subst_ren_utokens in aeq3; allsimpl; fold_terms.
-      unfold ren_atom in aeq3; allsimpl; boolvar; tcsp.
-      rw (ren_utokens_trivial [(get_fresh_atom t, a)] w) in aeq3;
-        [|simpl; apply disjoint_singleton_l; intro i; apply h4 in i;
-          apply get_fresh_atom_prop in i; sp]; GC.
-
-      eapply alpha_eq_trans in aeq3;[|exact aeq2]; clear aeq2.
-      apply alpha_eq_sym in aeq3.
-      eapply alpha_eq_trans in aeq3;[|exact q0]; clear q0.
-
-      dup ih1 as ih2.
-      eapply reduces_to_alpha in ih2;
-        [|apply nt_wf_subst; eauto 3 with slow;
-          apply nt_wf_eq; apply wf_subst_utokens; eauto 3 with slow
-         |apply alpha_eq_sym in aeq3; apply aeq3]; exrepnd.
-      rename t2' into s'.
-
-      exists s'; dands; eauto 2 with slow.
-      eapply reduces_to_if_split2;[exact q1|]; auto.
-Qed.
-
-Lemma alphaeq_preserves_wf_term_inv {o} :
-  forall (t1 t2 : @NTerm o),
-    alpha_eq t1 t2 -> wf_term t2 -> wf_term t1.
-Proof.
-  introv aeq wf; apply alpha_eq_sym in aeq; apply alphaeq_preserves_wf_term in aeq; auto.
-Qed.
-
-Lemma implies_alpha_eq_mk_lam {o} :
-  forall v (t1 t2 : @NTerm o),
-    alpha_eq t1 t2
-    -> alpha_eq (mk_lam v t1) (mk_lam v t2).
-Proof.
-  introv aeq.
-  unfold mk_fresh.
-  apply alpha_eq_oterm_combine; simpl; dands; auto.
-  introv i; repndors; cpx.
-  apply alpha_eq_bterm_congr; auto.
 Qed.
 
 
