computation/computation_preserves_diff_abs_bot.v
@@ -1,0 +1,1060 @@
+(*
+
+  Copyright 2014 Cornell University
+  Copyright 2015 Cornell University
+  Copyright 2016 Cornell University
+
+  This file is part of VPrl (the Verified Nuprl project).
+
+  VPrl is free software: you can redistribute it and/or modify
+  it under the terms of the GNU General Public License as published by
+  the Free Software Foundation, either version 3 of the License, or
+  (at your option) any later version.
+
+  VPrl is distributed in the hope that it will be useful,
+  but WITHOUT ANY WARRANTY; without even the implied warranty of
+  MERCHANTABILITY or FITNESS FOR A PARTICULAR PURPOSE.  See the
+  GNU General Public License for more details.
+
+  You should have received a copy of the GNU General Public License
+  along with VPrl.  If not, see <http://www.gnu.org/licenses/>.
+
+
+  Websites: http://nuprl.org/html/verification/
+            http://nuprl.org/html/Nuprl2Coq
+            https://github.com/vrahli/NuprlInCoq
+
+  Authors: Vincent Rahli
+
+*)
+
+
+
+Require Export computation8.
+Require Export computation11.
+Require Export computation_preserves_lib.
+Require Export atom_ren.
+Require Export alphaeq5.
+
+
+Lemma cl_sub_sub_find {o} :
+  forall (sub : @Sub o) v t,
+    sub_find sub v = Some t
+    -> cl_sub sub
+    -> closed t.
+Proof.
+  introv sf cl.
+  apply sub_find_some in sf.
+  eapply in_cl_sub; eauto.
+Qed.
+
+Inductive diff_abs_bot {o} : @NTerm o -> @NTerm o -> Type :=
+| diff_abs_bot_vterm : forall v, diff_abs_bot (vterm v) (vterm v)
+| diff_abs_bot_sterm :
+    forall f1 f2,
+      (forall n, diff_abs_bot (f1 n) (f2 n))
+      -> diff_abs_bot (sterm f1) (sterm f2)
+| diff_abs_bot_oterm :
+    forall op bs1 bs2,
+      length bs1 = length bs2
+      -> (forall b1 b2, LIn (b1,b2) (combine bs1 bs2) -> diff_abs_bot_b b1 b2)
+      -> diff_abs_bot (oterm op bs1) (oterm op bs2)
+| diff_abs_bot_abs :
+    forall abs bs v, diff_abs_bot (oterm (Abs abs) bs) (mk_vbot v)
+| diff_abs_bot_bot :
+    forall abs bs v, diff_abs_bot (mk_vbot v) (oterm (Abs abs) bs)
+with diff_abs_bot_b {o} : @BTerm o -> @BTerm o -> Type :=
+     | diff_abs_bot_bterm :
+         forall l t1 t2,
+           diff_abs_bot t1 t2
+           -> diff_abs_bot_b (bterm l t1) (bterm l t2).
+Hint Constructors diff_abs_bot.
+Hint Constructors diff_abs_bot_b.
+
+Ltac inv_diff_imp :=
+  match goal with
+  | [ H : forall _ _ : _, False -> _ |- _ ] => clear H
+  | [ H : forall _ _ : _, (?b1,?b2) = (_,_) [+] False -> _ |- _ ] =>
+    let h1 := fresh H in
+    assert (diff_abs_bot_b b1 b2) as h1 by (apply H; auto);
+      clear H
+  | [ H : forall _ _ : _, (?b1,?b2) = _ [+] (?b3,?b4) = _ [+] False -> _ |- _ ] =>
+    let h1 := fresh H in
+    let h2 := fresh H in
+    assert (diff_abs_bot_b b1 b2) as h1 by (apply H; auto);
+      assert (diff_abs_bot_b b3 b4) as h2 by (apply H; auto);
+      clear H
+  | [ H : forall _ _ : _, (?b1,?b2) = _ [+] (?b3,?b4) = _ [+] (?b5,?b6) = _ [+] False -> _ |- _ ] =>
+    let h1 := fresh H in
+    let h2 := fresh H in
+    let h3 := fresh H in
+    assert (diff_abs_bot_b b1 b2) as h1 by (apply H; auto);
+      assert (diff_abs_bot_b b3 b4) as h2 by (apply H; auto);
+      assert (diff_abs_bot_b b5 b6) as h3 by (apply H; auto);
+      clear H
+  | [ H : forall _ _ : _, (?b1,?b2) = _ [+] (?b3,?b4) = _ [+] LIn _ (combine ?bs1 ?bs2) -> _ |- _ ] =>
+    let h1 := fresh H in
+    let h2 := fresh H in
+    let h3 := fresh H in
+    let i  := fresh "i" in
+    assert (diff_abs_bot_b b1 b2) as h1 by (apply H; auto);
+      assert (diff_abs_bot_b b3 b4) as h2 by (apply H; auto);
+      assert (forall b1 b2, LIn (b1,b2) (combine bs1 bs2) -> diff_abs_bot_b b1 b2) as h3 by (introv i; apply H; auto);
+      clear H
+  end.
+
+Ltac inv_diff_len len :=
+  match type of len with
+  | S _ = length ?x => destruct x; simpl in len; cpx
+  | length ?x = S _ => destruct x; simpl in len; cpx
+  end.
+
+Ltac inv_diff_nterm H :=
+  let imp := fresh "imp" in
+  let len := fresh "len" in
+  inversion H as [|? ? imp|? ? ? len imp| |];
+    subst; clear H;
+    try (simpl in len; cpx; try (repeat (inv_diff_len len)));
+    try (simpl in imp; try inv_diff_imp).
+
+Ltac inv_diff_bterm H :=
+  let diff := fresh "diff" in
+  try (unfold nobnd in H);
+  inversion H as [? ? ? diff]; subst; clear H.
+
+Ltac inv_diff :=
+  match goal with
+  | [ H : diff_abs_bot (vterm _)   _ |- _ ] => inv_diff_nterm H
+  | [ H : diff_abs_bot (sterm _)   _ |- _ ] => inv_diff_nterm H
+  | [ H : diff_abs_bot (oterm _ _) _ |- _ ] => inv_diff_nterm H
+  | [ H : diff_abs_bot _ (vterm _)   |- _ ] => inv_diff_nterm H
+  | [ H : diff_abs_bot _ (sterm _)   |- _ ] => inv_diff_nterm H
+  | [ H : diff_abs_bot _ (oterm _ _) |- _ ] => inv_diff_nterm H
+  | [ H : diff_abs_bot_b (bterm _ _) _ |- _ ] => inv_diff_bterm H
+  | [ H : diff_abs_bot_b _ (bterm _ _) |- _ ] => inv_diff_bterm H
+
+  | [ H : diff_abs_bot_b (nobnd _) _ |- _ ] => inv_diff_bterm H
+  | [ H : diff_abs_bot_b _ (nobnd _) |- _ ] => inv_diff_bterm H
+
+  | [ H : diff_abs_bot (mk_nat _) _ |- _ ] => unfold mk_nat in H; inv_diff_nterm H
+  | [ H : diff_abs_bot _ (mk_nat _) |- _ ] => unfold mk_nat in H; inv_diff_nterm H
+  end.
+
+Ltac invdiff := repeat inv_diff.
+
+Definition diff_abs_bot_alpha {o} (t1 t2 : @NTerm o) :=
+  {u1 : NTerm
+   & {u2 : NTerm
+   & alpha_eq t1 u1
+   # alpha_eq t2 u2
+   # diff_abs_bot u1 u2}}.
+
+Lemma diff_abs_bot_implies_alpha {o} :
+  forall (t1 t2 : @NTerm o),
+    diff_abs_bot t1 t2
+    -> diff_abs_bot_alpha t1 t2.
+Proof.
+  introv diff.
+  eexists; eexists; dands; [| |eauto]; auto.
+Qed.
+Hint Resolve diff_abs_bot_implies_alpha : slow.
+
+Lemma diff_abs_bot_alpha_eapply {o} :
+  forall (a b c d : @NTerm o),
+    diff_abs_bot_alpha a c
+    -> diff_abs_bot_alpha b d
+    -> diff_abs_bot_alpha (mk_eapply a b) (mk_eapply c d).
+Proof.
+  introv d1 d2.
+  allunfold @diff_abs_bot_alpha; exrepnd.
+  eexists; eexists; dands;
+  try (apply implies_alpha_eq_mk_eapply);
+  try eassumption.
+  constructor; simpl; auto.
+  introv i; repndors; ginv; tcsp; constructor; auto.
+Qed.
+Hint Resolve diff_abs_bot_alpha_eapply : slow.
+
+Lemma diff_abs_bot_alpha_apply {o} :
+  forall (a b c d : @NTerm o),
+    diff_abs_bot_alpha a c
+    -> diff_abs_bot_alpha b d
+    -> diff_abs_bot_alpha (mk_apply a b) (mk_apply c d).
+Proof.
+  introv d1 d2.
+  allunfold @diff_abs_bot_alpha; exrepnd.
+  eexists; eexists; dands;
+  try (apply implies_alpha_eq_mk_apply);
+  try eassumption.
+  constructor; simpl; auto.
+  introv i; repndors; ginv; tcsp; constructor; auto.
+Qed.
+Hint Resolve diff_abs_bot_alpha_apply : slow.
+
+Lemma diff_abs_bot_alpha_fix {o} :
+  forall (a b : @NTerm o),
+    diff_abs_bot_alpha a b
+    -> diff_abs_bot_alpha (mk_fix a) (mk_fix b).
+Proof.
+  introv d.
+  allunfold @diff_abs_bot_alpha; exrepnd.
+  eexists; eexists; dands;
+  try (apply implies_alpha_eq_mk_fix);
+  try eassumption.
+  constructor; simpl; auto.
+  introv i; repndors; ginv; tcsp; constructor; auto.
+Qed.
+Hint Resolve diff_abs_bot_alpha_fix : slow.
+
+Lemma diff_abs_bot_preserves_isnoncan_like {o} :
+  forall (t1 t2 : @NTerm o),
+    isnoncan_like t1
+    -> diff_abs_bot t1 t2
+    -> isnoncan_like t2.
+Proof.
+  introv isn d.
+  inversion d; subst; try (unfold mk_vbot, mk_bottom, mk_fix); auto.
+Qed.
+Hint Resolve diff_abs_bot_preserves_isnoncan_like : slow.
+
+Lemma diff_abs_bot_sym {o} :
+  forall (t1 t2 : @NTerm o),
+    diff_abs_bot t1 t2
+    -> diff_abs_bot t2 t1.
+Proof.
+  nterm_ind t1 as [v|f ind|op bs ind] Case; introv d;
+  invdiff; auto; try (complete constructor).
+
+  Case "oterm".
+  constructor; auto.
+  introv i.
+  destruct b1 as [l1 t1].
+  destruct b2 as [l2 t2].
+  applydup @in_combine_swap in i; auto.
+  apply imp in i0.
+  inversion i0 as [? ? ? d]; clear i0; subst.
+  constructor.
+  apply in_combine in i; repnd.
+  eapply ind; eauto.
+Qed.
+Hint Resolve diff_abs_bot_sym : slow.
+
+Inductive diff_abs_bot_subs {o} : @Sub o -> @Sub o -> Type :=
+| dab_sub_nil : diff_abs_bot_subs [] []
+| dab_sub_cons :
+    forall v t1 t2 sub1 sub2,
+      diff_abs_bot t1 t2
+      -> diff_abs_bot_subs sub1 sub2
+      -> diff_abs_bot_subs ((v,t1) :: sub1) ((v,t2) :: sub2).
+Hint Constructors diff_abs_bot_subs.
+
+Lemma diff_abs_bot_subs_sub_find_some {o} :
+  forall (sub1 sub2 : @Sub o) v t,
+    diff_abs_bot_subs sub1 sub2
+    -> sub_find sub1 v = Some t
+    -> {u : NTerm & sub_find sub2 v = Some u # diff_abs_bot t u}.
+Proof.
+  induction sub1; destruct sub2; introv d fs; allsimpl; tcsp;
+  inversion d; subst.
+  boolvar; cpx.
+  eexists; eauto.
+Qed.
+
+Lemma diff_abs_bot_subs_sub_find_none {o} :
+  forall (sub1 sub2 : @Sub o) v,
+    diff_abs_bot_subs sub1 sub2
+    -> sub_find sub1 v = None
+    -> sub_find sub2 v = None.
+Proof.
+  induction sub1; destruct sub2; introv d fn; allsimpl; tcsp;
+  inversion d; subst.
+  boolvar; cpx.
+Qed.
+
+Lemma diff_abs_bot_subs_filter {o} :
+  forall (sub1 sub2 : @Sub o) l,
+    diff_abs_bot_subs sub1 sub2
+    -> diff_abs_bot_subs (sub_filter sub1 l) (sub_filter sub2 l).
+Proof.
+  induction sub1; destruct sub2; introv d; allsimpl; inversion d; auto.
+  boolvar; sp.
+Qed.
+Hint Resolve diff_abs_bot_subs_filter : slow.
+
+Lemma diff_abs_bot_lsubst_aux {o} :
+  forall (t1 t2 : @NTerm o) sub1 sub2,
+    diff_abs_bot t1 t2
+    -> diff_abs_bot_subs sub1 sub2
+    -> diff_abs_bot (lsubst_aux t1 sub1) (lsubst_aux t2 sub2).
+Proof.
+  nterm_ind1s t1 as [v|s|op bs ind] Case;
+  introv dt ds; allsimpl;
+  invdiff; allsimpl; auto;
+  try (complete (autorewrite with slow; constructor)).
+
+  - Case "vterm".
+    remember (sub_find sub1 v) as f1; symmetry in Heqf1; destruct f1.
+
+    + applydup (diff_abs_bot_subs_sub_find_some sub1 sub2) in Heqf1; auto.
+      exrepnd; allrw; auto.
+
+    + applydup (diff_abs_bot_subs_sub_find_none sub1 sub2) in Heqf1; auto.
+      allrw; auto.
+
+  - Case "oterm".
+    constructor; autorewrite with slow in *; auto.
+    introv i.
+    rewrite <- map_combine in i.
+    apply in_map_iff in i; exrepnd; allsimpl; ginv.
+    applydup imp in i1.
+    destruct a0 as [l1 t1].
+    destruct a as [l2 t2]; allsimpl.
+    invdiff.
+    constructor.
+    apply in_combine in i1; repnd.
+    eapply ind; eauto 2 with slow.
+Qed.
+
+Lemma diff_abs_bot_alpha_l {o} :
+  forall (t1 t2 t3 : @NTerm o),
+    alpha_eq t1 t2
+    -> diff_abs_bot_alpha t2 t3
+    -> diff_abs_bot_alpha t1 t3.
+Proof.
+  introv aeq d.
+  allunfold @diff_abs_bot_alpha; exrepnd.
+  exists u1 u2; dands; eauto 3 with slow.
+Qed.
+
+Lemma diff_abs_bot_alpha_r {o} :
+  forall (t1 t2 t3 : @NTerm o),
+    diff_abs_bot_alpha t1 t2
+    -> alpha_eq t2 t3
+    -> diff_abs_bot_alpha t1 t3.
+Proof.
+  introv d aeq.
+  allunfold @diff_abs_bot_alpha; exrepnd.
+  exists u1 u2; dands; eauto 3 with slow.
+Qed.
+
+Definition diff_abs_bot_bterms {o} (bs1 bs2 : list (@BTerm o)) :=
+  br_bterms diff_abs_bot_b bs1 bs2.
+
+Lemma diff_abs_bot_refl {o} :
+  forall (t : @NTerm o),
+    diff_abs_bot t t.
+Proof.
+  nterm_ind t as [v|s ind|op bs ind] Case; introv; allsimpl; auto.
+
+  Case "oterm".
+  constructor; auto.
+  introv i.
+  rw in_combine_same in i; repnd; subst.
+  destruct b2 as [l t].
+  constructor; eapply ind; eauto.
+Qed.
+Hint Resolve diff_abs_bot_refl : slow.
+
+Lemma diff_abs_bot_subs_refl {o} :
+  forall (sub : @Sub o),
+    diff_abs_bot_subs sub sub.
+Proof.
+  induction sub; introv; allsimpl; auto.
+  destruct a.
+  constructor; eauto 3 with slow.
+Qed.
+Hint Resolve diff_abs_bot_subs_refl : slow.
+
+Lemma alpha_eq_mk_vbot_implies {o} :
+  forall v (t : @NTerm o),
+    alpha_eq (mk_vbot v) t
+    -> {z : NVar & t = mk_vbot z}.
+Proof.
+  introv aeq.
+  inversion aeq as [|?|? ? ? len imp]; subst; allsimpl; cpx; clear aeq.
+  pose proof (imp 0) as h; clear imp; autodimp h hyp.
+  unfold selectbt in h; allsimpl.
+  apply alphaeqbt_nilv in h; exrepnd; subst.
+  inversion h0 as [|?|? ? ? len imp]; subst; allsimpl; cpx; clear h0.
+  pose proof (imp 0) as h; clear imp; autodimp h hyp.
+  unfold selectbt in h; allsimpl.
+  apply alphaeqbt_1v in h; exrepnd; subst; allrw disjoint_singleton_l.
+  allunfold @lsubst; allsimpl.
+  allrw not_over_or; repnd; boolvar; allrw disjoint_singleton_r.
+  - destruct nt2 as [w|f|op bs]; allsimpl; allrw not_over_or; repnd; boolvar; tcsp;
+    inversion h0; subst; tcsp.
+    exists w; auto.
+  - destruct n; allunfold @all_vars; allrw in_app_iff; sp.
+Qed.
+
+Lemma diff_abs_bot_change_bound_vars {o} :
+  forall vs (t1 t2 : @NTerm o),
+    diff_abs_bot t1 t2
+    -> {u1 : NTerm
+        & {u2 : NTerm
+        & diff_abs_bot u1 u2
+        # alpha_eq t1 u1
+        # alpha_eq t2 u2
+        # disjoint (bound_vars u1) vs
+        # disjoint (bound_vars u2) vs}}.
+Proof.
+  nterm_ind1s t1 as [v|s ind|op bs ind] Case; introv d;
+  invdiff; allsimpl; auto.
+
+  - Case "vterm".
+    exists (@mk_var o v) (@mk_var o v); simpl; dands; eauto 3 with slow.
+
+  - Case "sterm".
+    exists (sterm s) (sterm f2); dands; simpl; auto.
+
+  - Case "oterm".
+
+    assert ({bs' : list BTerm
+             & {bs2' : list BTerm
+             & alpha_eq_bterms bs bs'
+             # alpha_eq_bterms bs2 bs2'
+             # diff_abs_bot_bterms bs' bs2'
+             # disjoint (flat_map bound_vars_bterm bs') vs
+             # disjoint (flat_map bound_vars_bterm bs2') vs}}) as h.
+
+      { revert dependent bs2.
+        induction bs; destruct bs2; introv len imp; allsimpl; ginv.
+        - exists ([] : list (@BTerm o)) ([] : list (@BTerm o));
+            dands; simpl; eauto 3 with slow; try (apply br_bterms_nil).
+        - cpx.
+          destruct a as [l1 t1].
+          destruct b as [l2 t2].
+          pose proof (imp (bterm l1 t1) (bterm l2 t2)) as h; autodimp h hyp.
+          invdiff.
+          pose proof (ind t1 t1 l2) as h; repeat (autodimp h hyp); eauto 3 with slow.
+          pose proof (h t2 diff) as k; clear h.
+          exrepnd.
+
+          autodimp IHbs hyp.
+          { introv i d; eapply ind; eauto. }
+          pose proof (IHbs bs2) as k.
+          repeat (autodimp k hyp).
+          exrepnd.
+
+          pose proof (fresh_vars
+                        (length l2)
+                        (vs
+                           ++ l2
+                           ++ all_vars t1
+                           ++ all_vars t2
+                           ++ all_vars u1
+                           ++ all_vars u2
+                        )) as fv; exrepnd.
+          allrw disjoint_app_r; repnd.
+
+          exists ((bterm lvn (lsubst_aux u1 (var_ren l2 lvn))) :: bs')
+                 ((bterm lvn (lsubst_aux u2 (var_ren l2 lvn))) :: bs2');
+            dands; simpl;
+            try (apply br_bterms_cons);
+            try (apply alpha_eq_bterm_congr);
+            tcsp.
+          { apply alpha_bterm_change_aux; eauto 3 with slow.
+            allrw disjoint_app_l; dands; eauto 3 with slow. }
+          { apply alpha_bterm_change_aux; eauto 3 with slow.
+            allrw disjoint_app_l; dands; eauto 3 with slow. }
+          { constructor.
+            apply diff_abs_bot_lsubst_aux; eauto 3 with slow;
+            try (rw @sub_free_vars_var_ren; eauto 3 with slow);
+            try (rw @dom_sub_var_ren; eauto 3 with slow). }
+          { allrw disjoint_app_l; dands; eauto 3 with slow.
+            pose proof (subvars_bound_vars_lsubst_aux
+                          u1 (var_ren l2 lvn)) as sv.
+            eapply subvars_disjoint_l;[exact sv|].
+            apply disjoint_app_l; dands; auto.
+            rw @sub_bound_vars_var_ren; auto. }
+          { allrw disjoint_app_l; dands; eauto 3 with slow.
+            pose proof (subvars_bound_vars_lsubst_aux
+                          u2 (var_ren l2 lvn)) as sv.
+            eapply subvars_disjoint_l;[exact sv|].
+            apply disjoint_app_l; dands; auto.
+            rw @sub_bound_vars_var_ren; auto. }
+      }
+
+      exrepnd.
+      allunfold @alpha_eq_bterms.
+      allunfold @diff_abs_bot_bterms.
+      allunfold @br_bterms.
+      allunfold @br_list; repnd.
+      exists (oterm op bs') (oterm op bs2'); dands;
+      eauto 3 with slow;
+      try (complete (apply alpha_eq_oterm_combine; dands; auto)).
+
+  - pose proof (change_bvars_alpha_wspec vs (oterm (Abs abs) bs)) as p.
+    exrepnd.
+    pose proof (change_bvars_alpha_wspec vs (@mk_vbot o v)) as q.
+    exrepnd.
+    eexists; eexists; dands; try (exact p0); try (exact q0);
+    eauto 3 with slow.
+
+    apply alpha_eq_mk_vbot_implies in q0; exrepnd; subst.
+    inversion p0; subst; auto.
+
+  - pose proof (change_bvars_alpha_wspec vs (oterm (Abs abs) bs0)) as p.
+    exrepnd.
+    pose proof (change_bvars_alpha_wspec vs (@mk_vbot o v)) as q.
+    exrepnd.
+    eexists; eexists; dands; try (exact p0); try (exact q0);
+    eauto 3 with slow.
+
+    apply alpha_eq_mk_vbot_implies in q0; exrepnd; subst.
+    inversion p0; subst; auto.
+Qed.
+
+XXXXXXXXXXXXXX
+
+Lemma diff_abs_bot_lsubst {o} :
+  forall (t1 t2 : @NTerm o) sub1 sub2,
+    diff_abs_bot t1 t2
+    -> diff_abs_bot_subs sub1 sub2
+    -> diff_abs_bot_alpha (lsubst t1 sub1) (lsubst t2 sub2).
+Proof.
+  introv d1 d2.
+
+  pose proof (change_bvars_alpha_wspec (sub_free_vars sub1) t1) as h.
+  destruct h as [t1' h]; repnd.
+
+  pose proof (change_bvars_alpha_wspec (sub_free_vars sub2) t2) as q.
+  destruct q as [t2' q]; repnd.
+
+  eapply diff_abs_bot_alpha_l;[apply lsubst_alpha_congr2;exact h|].
+  eapply diff_abs_bot_alpha_r;[|apply alpha_eq_sym;apply lsubst_alpha_congr2;exact q].
+
+  pose proof (unfold_lsubst sub1 t1') as z; exrepnd.
+  rewrite z0; clear z0.
+
+  pose proof (unfold_lsubst sub2 t2) as q; exrepnd.
+  rewrite q0; clear q0.
+
+  exists (lsubst_aux t1 sub1) (lsubst_aux t2 sub2).
+
+  apply diff_abs_bot_lsubst_aux; auto.
+
+Qed.
+
+Lemma compute_step_abs2bot_lsubst_aux {o} :
+  forall (t : @NTerm o) t' u,
+    wf_term t
+    -> compute_step [] t = csuccess u
+    -> diff_abs_bot t t'
+    -> {u' : NTerm
+        & compute_step [] t' = csuccess u'
+        # diff_abs_bot_alpha u u'}.
+Proof.
+  nterm_ind1s t as [v|f ind|op bs ind] Case; introv wf comp diff.
+
+  - Case "vterm".
+    allsimpl; ginv.
+
+  - Case "sterm".
+    csunf comp; allsimpl; ginv; auto.
+    inv_diff.
+    csunf; simpl.
+    eexists; dands; eauto 3 with slow.
+
+  - Case "oterm".
+    dopid op as [can|ncan|exc|abs] SCase.
+
+    + SCase "Can".
+      csunf comp; allsimpl; ginv; auto.
+      inv_diff.
+      eexists; csunf; simpl; dands; eauto 3 with slow.
+
+    + SCase "NCan".
+      destruct bs as [|b1 bs]; try (complete (allsimpl; ginv)).
+      destruct b1 as [l t]; try (complete (allsimpl; ginv)).
+      destruct l; try (complete (allsimpl; ginv)).
+
+      {
+        destruct t as [x|f|op bts]; try (complete (allsimpl; ginv));[|].
+
+        - csunf comp; allsimpl.
+          dopid_noncan ncan SSCase; allsimpl; ginv; auto.
+
+          {
+            SSCase "NApply".
+            apply compute_step_seq_apply_success in comp; exrepnd; subst; allsimpl.
+            csunf; simpl; auto.
+            invdiff.
+            simpl.
+            eexists; dands; eauto 5 with slow.
+          }
+
+          {
+            SSCase "NEApply".
+
+            apply compute_step_eapply_success in comp; exrepnd; subst.
+            repndors; exrepnd; allsimpl; subst.
+
+            + apply compute_step_eapply2_success in comp1; repnd; subst.
+              repndors; exrepnd; subst; ginv.
+              invdiff.
+              csunf; simpl.
+              dcwf h; simpl.
+              boolvar; try omega.
+              rewrite Znat.Nat2Z.id; auto.
+              eexists; dands; eauto 2 with slow.
+
+            + invdiff.
+              csunf; simpl.
+              apply isexc_implies2 in comp0; exrepnd; subst.
+              invdiff.
+              dcwf h; simpl; auto.
+              eexists; dands; eauto 3 with slow.
+
+            + invdiff.
+              fold_terms.
+              rewrite compute_step_eapply_iscan_isnoncan_like; eauto 3 with slow.
+              pose proof (ind arg2 arg2 []) as h; clear ind.
+              repeat (autodimp h hyp); eauto 3 with slow.
+              apply wf_term_eapply_iff in wf; exrepnd; allunfold @nobnd; ginv.
+              eapply h in comp1; clear h; auto; try(exact diff).
+              exrepnd; rewrite comp1.
+              allsimpl; cpx.
+              eexists; dands; eauto.
+              fold_terms; eauto 4 with slow.
+          }
+
+          {
+            SSCase "NFix".
+            apply compute_step_fix_success in comp; repnd; subst.
+            invdiff.
+            csunf; simpl; auto.
+            eexists; dands; eauto.
+            fold_terms; eauto 7 with slow.
+          }
+
+          {
+            SSCase "NCbv".
+            apply compute_step_cbv_success in comp; exrepnd; subst.
+            invdiff.
+            csunf; simpl; auto.
+            eexists; dands; eauto.
+            eapply alpha_eq_trans;[|apply alpha_eq_sym; apply abs2bot_lsubst]; auto.
+          }
+
+          {
+            SSCase "NTryCatch".
+            apply compute_step_try_success in comp; exrepnd; subst; allsimpl.
+            csunf; simpl.
+            eexists; dands; eauto.
+          }
+
+          {
+            SSCase "NCanTest".
+            apply compute_step_seq_can_test_success in comp; exrepnd; subst; allsimpl.
+            csunf; simpl.
+            eexists; dands; eauto.
+          }
+
+        - dopid op as [can2|ncan2|exc2|abs2] SSCase.
+
+          + SSCase "Can".
+            dopid_noncan ncan SSSCase.
+
+            {
+              SSSCase "NApply".
+
+              csunf comp; allsimpl.
+              apply compute_step_apply_success in comp.
+              repndors; exrepnd; subst; auto; csunf; simpl; eexists; dands; eauto.
+              eapply alpha_eq_trans;[|apply alpha_eq_sym; apply abs2bot_lsubst]; auto.
+            }
+
+            {
+              SSSCase "NEApply".
+
+              csunf comp; allsimpl.
+              apply compute_step_eapply_success in comp.
+              repndors; exrepnd; subst; auto.
+              repndors; exrepnd; subst; allsimpl; auto.
+
+              - apply compute_step_eapply2_success in comp1; repnd; subst.
+                repndors; exrepnd; subst; auto; ginv.
+
+                + unfold mk_lam in *; ginv.
+                  csunf; simpl.
+                  dcwf h; simpl.
+                  apply iscan_implies in comp0; repndors; exrepnd; subst; simpl; auto;
+                  eexists; dands; eauto;
+                  eapply alpha_eq_trans;
+                  try (apply alpha_eq_sym; apply abs2bot_lsubst); auto.
+
+                + unfold mk_nseq in *; allsimpl; ginv; GC.
+                  csunf; simpl.
+                  dcwf h; simpl.
+                  boolvar; simpl; auto; try omega.
+                  rewrite Znat.Nat2Z.id; auto.
+                  eexists; dands; eauto.
+
+              - fold_terms; rewrite compute_step_eapply_iscan_isexc; eauto 3 with slow.
+
+              - fold_terms; rewrite compute_step_eapply_iscan_isnoncan_like; eauto 3 with slow.
+
+                pose proof (ind arg2 arg2 []) as q; clear ind.
+                repeat (autodimp q hyp); eauto 2 with slow.
+                apply wf_term_eapply_iff in wf; exrepnd; allunfold @nobnd; ginv.
+                apply q in comp1; clear q; auto.
+                exrepnd; rewrite comp1; auto.
+                eexists; dands; eauto.
+                repeat prove_alpha_eq4.
+            }
+
+            {
+              SSSCase "NFix".
+
+              csunf comp; allsimpl.
+              apply compute_step_fix_success in comp.
+              repndors; exrepnd; subst; auto.
+              csunf; simpl; eexists; dands; eauto.
+            }
+
+            {
+              SSSCase "NSpread".
+
+              csunf comp; allsimpl.
+              apply compute_step_spread_success in comp.
+              repndors; exrepnd; subst; auto.
+              csunf; simpl; eexists; dands; eauto.
+              eapply alpha_eq_trans;[|apply alpha_eq_sym; apply abs2bot_lsubst]; auto.
+            }
+
+            {
+              SSSCase "NDsup".
+
+              csunf comp; allsimpl.
+              apply compute_step_dsup_success in comp.
+              repndors; exrepnd; subst; auto.
+              csunf; simpl; eexists; dands; eauto.
+              eapply alpha_eq_trans;[|apply alpha_eq_sym; apply abs2bot_lsubst]; auto.
+            }
+
+            {
+              SSSCase "NDecide".
+
+              csunf comp; allsimpl.
+              apply compute_step_decide_success in comp.
+              repndors; exrepnd; subst; auto.
+              repndors; exrepnd; subst; auto;
+              csunf; simpl; eexists; dands; eauto;
+              eapply alpha_eq_trans;
+              try (apply alpha_eq_sym; apply abs2bot_lsubst); auto.
+            }
+
+            {
+              SSSCase "NCbv".
+
+              csunf comp; allsimpl.
+              apply compute_step_cbv_success in comp.
+              repndors; exrepnd; subst; auto.
+              csunf; simpl; eexists; dands; eauto.
+              eapply alpha_eq_trans;
+                try (apply alpha_eq_sym; apply abs2bot_lsubst); auto.
+            }
+
+            {
+              SSSCase "NSleep".
+
+              csunf comp; allsimpl.
+              apply compute_step_sleep_success in comp.
+              repndors; exrepnd; subst; auto.
+              csunf; simpl.
+              unfold compute_step_sleep; simpl.
+              eexists; dands; eauto.
+            }
+
+            {
+              SSSCase "NTUni".
+
+              csunf comp; allsimpl.
+              apply compute_step_tuni_success in comp.
+              repndors; exrepnd; subst; auto.
+              csunf; simpl.
+              unfold compute_step_tuni; simpl.
+              boolvar; try omega.
+              rewrite Znat.Nat2Z.id; auto.
+              eexists; dands; eauto.
+            }
+
+            {
+              SSSCase "NMinus".
+
+              csunf comp; allsimpl.
+              apply compute_step_minus_success in comp.
+              repndors; exrepnd; subst; auto.
+              csunf; simpl.
+              unfold compute_step_minus; simpl.
+              eexists; dands; eauto.
+            }
+
+            {
+              SSSCase "NFresh".
+
+              csunf comp; allsimpl; ginv.
+            }
+
+            {
+              SSSCase "NTryCatch".
+
+              csunf comp; allsimpl.
+              apply compute_step_try_success in comp.
+              repndors; exrepnd; subst; auto.
+              csunf; simpl.
+              eexists; dands; eauto.
+            }
+
+            {
+              SSSCase "NParallel".
+
+              csunf comp; allsimpl.
+              apply compute_step_parallel_success in comp.
+              repndors; exrepnd; subst; auto.
+              csunf; simpl.
+              unfold compute_step_parallel.
+              eexists; dands; eauto.
+            }
+
+            {
+              SSSCase "NCompOp".
+
+              apply compute_step_ncompop_can1_success in comp; repnd.
+              repndors; exrepnd; allsimpl; subst; tcsp; simpl.
+
+              - csunf; simpl.
+                dcwf h.
+                apply compute_step_compop_success_can_can in comp1; exrepnd; subst; ginv; GC.
+                repndors; exrepnd; subst; allsimpl;
+                unfold compute_step_comp; allrw;
+                eexists; dands; eauto;
+                boolvar; auto.
+
+              - rewrite compute_step_ncompop_ncanlike2; eauto 3 with slow.
+                dcwf h.
+                pose proof (ind t t []) as q; clear ind.
+                repeat (autodimp q hyp); eauto 2 with slow.
+                allrw @wf_term_ncompop_iff; exrepnd; ginv.
+                apply q in comp4; clear q; auto.
+                exrepnd.
+                rewrite comp2; auto.
+                eexists; dands; eauto.
+                repeat prove_alpha_eq4.
+
+              - csunf; simpl.
+                apply isexc_implies2 in comp1; exrepnd; subst.
+                dcwf h; simpl; auto.
+                eexists; dands; eauto.
+            }
+
+            {
+              SSSCase "NArithOp".
+
+              apply compute_step_narithop_can1_success in comp; repnd.
+              repndors; exrepnd; allsimpl; subst; tcsp; allsimpl.
+
+              - csunf; simpl.
+                dcwf h.
+                apply compute_step_arithop_success_can_can in comp1; exrepnd; subst; ginv; GC.
+                repndors; exrepnd; subst; allsimpl;
+                unfold compute_step_comp; allrw;
+                eexists; dands; eauto;
+                boolvar; auto.
+
+              - rewrite compute_step_narithop_ncanlike2; eauto 3 with slow.
+                dcwf h.
+                pose proof (ind t t []) as q; clear ind.
+                repeat (autodimp q hyp); eauto 2 with slow.
+                allrw @wf_term_narithop_iff; exrepnd; ginv.
+                apply q in comp4; clear q; auto.
+                exrepnd.
+                rewrite comp2; auto.
+                eexists; dands; eauto.
+                repeat prove_alpha_eq4.
+
+              - csunf; simpl.
+                apply isexc_implies2 in comp1; exrepnd; subst.
+                dcwf h; simpl; auto.
+                eexists; dands; eauto.
+            }
+
+            {
+              SSSCase "NCanTest".
+
+              csunf comp; allsimpl.
+              apply compute_step_can_test_success in comp.
+              repndors; exrepnd; subst; auto.
+              csunf; simpl.
+              eexists; dands; eauto.
+              destruct (canonical_form_test_for c can2); auto.
+            }
+
+          + SSCase "NCan".
+
+            csunf comp; allsimpl.
+            remember (compute_step [] (oterm (NCan ncan2) bts)) as c.
+            destruct c; allsimpl; ginv.
+            symmetry in Heqc.
+
+            pose proof (ind
+                          (oterm (NCan ncan2) bts)
+                          (oterm (NCan ncan2) bts) []) as q; clear ind.
+            repeat (autodimp q hyp); eauto 2 with slow.
+
+            applydup @wf_oterm_iff in wf; repnd.
+            pose proof (wf0 (bterm [] (oterm (NCan ncan2) bts))) as wfn; allsimpl.
+            autodimp wfn hyp.
+            allrw @wf_bterm_iff.
+
+            apply q in Heqc; clear q; auto.
+            exrepnd.
+            csunf; allsimpl.
+            rewrite Heqc1; auto; simpl.
+            eexists; dands; eauto.
+            repeat prove_alpha_eq4.
+
+          + SSCase "Exc".
+
+            csunf comp; allsimpl.
+            apply compute_step_catch_success in comp.
+            repndors; exrepnd; subst; allsimpl; ginv.
+
+            * csunf; simpl; auto.
+              eexists; dands; eauto.
+              unfold mk_atom_eq.
+              repeat prove_alpha_eq4.
+              eapply alpha_eq_trans;
+                try (apply alpha_eq_sym; apply abs2bot_lsubst); auto.
+
+            * csunf; simpl; auto.
+              rewrite compute_step_catch_if_diff; auto.
+              eexists; dands; eauto.
+
+          + SSCase "Abs".
+
+            csunf comp; allsimpl; ginv.
+      }
+
+      {
+        csunf comp; allsimpl.
+        apply compute_step_fresh_success in comp; exrepnd; subst.
+        repndors; exrepnd; subst; ginv.
+
+        - csunf; simpl; boolvar; auto.
+          eexists; dands; eauto.
+
+        - rewrite compute_step_fresh_if_isvalue_like2; simpl; eauto 3 with slow.
+          eexists; dands; eauto.
+          apply pushdown_fresh_abs2bot; auto.
+
+        - rewrite compute_step_fresh_if_isnoncan_like; simpl; eauto 3 with slow.
+
+          allrw @wf_fresh_iff.
+
+          pose proof (ind t (subst t n (mk_utoken (get_fresh_atom t))) [n]) as q; clear ind.
+          repeat (autodimp q hyp); eauto 2 with slow.
+          { rewrite simple_osize_subst; eauto 2 with slow. }
+          apply q in comp2; clear q; eauto 3 with slow;[].
+          exrepnd; allsimpl.
+
+          pose proof (abs2bot_lsubst t [(n,mk_utoken (get_fresh_atom t))]) as aeq.
+          pose proof (compute_step_alpha
+                        []
+                        (abs2bot (lsubst t [(n, mk_utoken (get_fresh_atom t))]))
+                        (lsubst (abs2bot t) (abs2bot_sub [(n, mk_utoken (get_fresh_atom t))]))
+                        w) as comp.
+          repeat (autodimp comp hyp).
+          { apply implies_nt_wf_abs2bot.
+            apply nt_wf_subst; eauto 2 with slow. }
+          exrepnd; allsimpl.
+          fold_terms; allrw @fold_subst.
+
+          assert (!LIn (get_fresh_atom t) (get_utokens (abs2bot t))) as ni1.
+          {
+            intro h.
+            pose proof (implies_props_abs2bot t) as q; repnd.
+            apply q in h.
+            apply get_fresh_atom_prop in h; tcsp.
+          }
+
+          assert (!LIn (get_fresh_atom (abs2bot t)) (get_utokens (abs2bot t))) as ni2.
+          {
+            intro h.
+            apply get_fresh_atom_prop in h; tcsp.
+          }
+
+          pose proof (compute_step_subst_utoken
+                        []
+                        (abs2bot t)
+                        t2'
+                        [(n, mk_utoken (get_fresh_atom t))]) as comp'.
+          repeat (autodimp comp' hyp); simpl; eauto 3 with slow.
+
+          { unfold get_utokens_sub; simpl.
+            apply disjoint_singleton_l; auto. }
+
+          exrepnd; allsimpl.
+
+          pose proof (comp'0 [(n, mk_utoken (get_fresh_atom (abs2bot t)))]) as comp''.
+          allsimpl.
+          repeat (autodimp comp'' hyp); eauto 3 with slow.
+
+          { unfold get_utokens_sub; simpl.
+            apply disjoint_singleton_l; auto. }
+
+          exrepnd; allsimpl.
+          allrw @fold_subst.
+          rewrite comp''1; simpl.
+          eexists; dands; eauto.
+
+          apply implies_alpha_eq_mk_fresh.
+
+          rename comp''0 into aeq1.
+          assert (alpha_eq (subst w0 n (mk_utoken (get_fresh_atom t))) (abs2bot x)) as aeq2.
+          { eauto 4 with slow. }
+
+          unfold get_utokens_sub in *; allsimpl.
+          allrw disjoint_singleton_l.
+
+          eapply alpha_eq_trans;
+            [|apply alpha_eq_sym; apply abs2bot_subst_utokens].
+          simpl.
+
+          eapply alpha_eq_trans;
+            [apply alpha_eq_subst_utokens_same;exact aeq1|].
+
+          eapply alpha_eq_trans;
+            [apply simple_alphaeq_subst_utokens_subst;
+              intro i; apply comp'4 in i; auto|].
+
+          eapply alpha_eq_trans;
+            [|apply alpha_eq_subst_utokens_same;exact aeq2].
+
+          eapply alpha_eq_trans;
+            [|apply alpha_eq_sym;apply simple_alphaeq_subst_utokens_subst;auto].
+
+          auto.
+      }
+
+    + SCase "Exc".
+
+      csunf comp; allsimpl; ginv.
+      csunf; simpl.
+      eexists; dands; eauto.
+
+    + SCase "Abs".
+
+      csunf comp; allsimpl.
+      apply compute_step_lib_success in comp.
+      exrepnd; subst.
+      unfold found_entry in comp0; allsimpl; ginv.
+Qed.
+
+
+(*
+*** Local Variables:
+*** coq-load-path: ("." "../util/" "../terms/")
+*** End:
+*)
